<?xml version="1.0"?>
<rdf:RDF xmlns="http://www.w3id.org/eurocodes/ec1990#"
     xml:base="http://www.w3id.org/eurocodes/ec1990"
     xmlns:ns="http://www.w3.org/2003/06/sw-vocab-status/ns#"
     xmlns:ns1="http://creativecommons.org/ns#"
     xmlns:ns2="http://www.w3.org/2006/vcard/ns#"
     xmlns:owl="http://www.w3.org/2002/07/owl#"
     xmlns:rdf="http://www.w3.org/1999/02/22-rdf-syntax-ns#"
     xmlns:xml="http://www.w3.org/XML/1998/namespace"
     xmlns:xsd="http://www.w3.org/2001/XMLSchema#"
     xmlns:rdfs="http://www.w3.org/2000/01/rdf-schema#"
     xmlns:skos="http://www.w3.org/2004/02/skos/core#"
     xmlns:vann="http://purl.org/vocab/vann/"
     xmlns:terms="http://purl.org/dc/terms/"
     xmlns:schema="https://schema.org/">
    <owl:Ontology rdf:about="http://www.w3id.org/eurocodes/ec1990#">
        <owl:imports rdf:resource="https://www.w3id.org/bot"/>
        <ns1:license>http://creativecommons.org/licenses/by/3.0/</ns1:license>
        <terms:contributor>Daniel V. Oliveira (danvco@civil.uminho.pt)</terms:contributor>
        <terms:contributor>José Granja (granja@civil.uminho.pt)</terms:contributor>
        <terms:contributor>Miguel Azenha (miguel.azenha@civil.uminho.pt)</terms:contributor>
        <terms:contributor>Rolando Chacón (rolando.chacon@upc.edu)</terms:contributor>
        <terms:creator>Agnieszka Jędrzejewska (agnieszka.jedrzejewska@polsl.pl), Maria Laura Leonardi (mlauraleonardi@gmail.com), Carlos Ramonell Cazador (carlos.ramonell@upc.edu)</terms:creator>
        <terms:date rdf:datatype="http://www.w3.org/2001/XMLSchema#date">2025-06-30</terms:date>
        <terms:description>Core ontology formalising knowledge from Eurocode 0 for automated structural design and verification</terms:description>
        <terms:format>ttl</terms:format>
        <terms:language>en</terms:language>
        <terms:modified rdf:datatype="http://www.w3.org/2001/XMLSchema#date">2025-06-30</terms:modified>
        <terms:title>ECO - Eurocode Core Ontology</terms:title>
        <vann:preferredNamespacePrefix>ec</vann:preferredNamespacePrefix>
        <vann:preferredNamespaceUri>http://www.w3id.org/eurocodes/ec1990#</vann:preferredNamespaceUri>
        <owl:versionInfo>1.0.0</owl:versionInfo>
        <skos:hasTopConcept rdf:resource="http://www.w3id.org/eurocodes/ec1990#Action"/>
        <skos:hasTopConcept rdf:resource="http://www.w3id.org/eurocodes/ec1990#CombinationOfActions"/>
        <skos:hasTopConcept rdf:resource="http://www.w3id.org/eurocodes/ec1990#ConstructionWork"/>
        <skos:hasTopConcept rdf:resource="http://www.w3id.org/eurocodes/ec1990#DesignSituation"/>
        <skos:hasTopConcept rdf:resource="http://www.w3id.org/eurocodes/ec1990#EffectOfAction"/>
        <skos:hasTopConcept rdf:resource="http://www.w3id.org/eurocodes/ec1990#LimitState"/>
    </owl:Ontology>
    


    <!-- 
    ///////////////////////////////////////////////////////////////////////////////////////
    //
    // Annotation properties
    //
    ///////////////////////////////////////////////////////////////////////////////////////
     -->


    


    <!-- http://creativecommons.org/ns#license -->


    <owl:AnnotationProperty rdf:about="http://creativecommons.org/ns#license"/>
    


    <!-- http://purl.org/dc/terms/date -->


    <owl:AnnotationProperty rdf:about="http://purl.org/dc/terms/date"/>
    


    <!-- http://purl.org/dc/terms/format -->


    <owl:AnnotationProperty rdf:about="http://purl.org/dc/terms/format"/>
    


    <!-- http://purl.org/dc/terms/language -->


    <owl:AnnotationProperty rdf:about="http://purl.org/dc/terms/language"/>
    


    <!-- http://purl.org/dc/terms/source -->


    <owl:AnnotationProperty rdf:about="http://purl.org/dc/terms/source"/>
    


    <!-- http://www.w3.org/2004/02/skos/core#altLabel -->


    <owl:AnnotationProperty rdf:about="http://www.w3.org/2004/02/skos/core#altLabel"/>
    


    <!-- http://www.w3.org/2004/02/skos/core#definition -->


    <owl:AnnotationProperty rdf:about="http://www.w3.org/2004/02/skos/core#definition"/>
    


    <!-- http://www.w3.org/2004/02/skos/core#editorialNote -->


    <owl:AnnotationProperty rdf:about="http://www.w3.org/2004/02/skos/core#editorialNote"/>
    


    <!-- http://www.w3.org/2004/02/skos/core#example -->


    <owl:AnnotationProperty rdf:about="http://www.w3.org/2004/02/skos/core#example"/>
    


    <!-- http://www.w3.org/2004/02/skos/core#hasTopConcept -->


    <owl:AnnotationProperty rdf:about="http://www.w3.org/2004/02/skos/core#hasTopConcept"/>
    


    <!-- http://www.w3.org/2004/02/skos/core#scopeNote -->


    <owl:AnnotationProperty rdf:about="http://www.w3.org/2004/02/skos/core#scopeNote"/>
    


    <!-- 
    ///////////////////////////////////////////////////////////////////////////////////////
    //
    // Datatypes
    //
    ///////////////////////////////////////////////////////////////////////////////////////
     -->


    


    <!-- http://www.w3.org/2001/XMLSchema#date -->


    <rdfs:Datatype rdf:about="http://www.w3.org/2001/XMLSchema#date"/>
    


    <!-- 
    ///////////////////////////////////////////////////////////////////////////////////////
    //
    // Object Properties
    //
    ///////////////////////////////////////////////////////////////////////////////////////
     -->


    


    <!-- http://qudt.org/3.1.2/schema/qudt/quantityValue -->


    <owl:ObjectProperty rdf:about="http://qudt.org/3.1.2/schema/qudt/quantityValue"/>
    


    <!-- http://www.w3id.org/eurocodes/ec1990#appliesTo -->


    <owl:ObjectProperty rdf:about="http://www.w3id.org/eurocodes/ec1990#appliesTo">
        <rdfs:domain rdf:resource="http://www.w3id.org/eurocodes/ec1990#Action"/>
        <rdfs:range rdf:resource="http://www.w3id.org/eurocodes/ec1990#StructuralMember"/>
        <rdfs:label xml:lang="en">applies to</rdfs:label>
        <skos:definition>Relates an action to the structural member or structure it acts upon.</skos:definition>
    </owl:ObjectProperty>
    


    <!-- http://www.w3id.org/eurocodes/ec1990#causesEffect -->


    <owl:ObjectProperty rdf:about="http://www.w3id.org/eurocodes/ec1990#causesEffect">
        <rdfs:domain rdf:resource="http://www.w3id.org/eurocodes/ec1990#CombinationOfActions"/>
        <rdfs:range rdf:resource="http://www.w3id.org/eurocodes/ec1990#EffectOfAction"/>
        <rdfs:label xml:lang="en">causes effect</rdfs:label>
        <skos:definition>Relates a combination of actions to the effects it causes in the structure.</skos:definition>
    </owl:ObjectProperty>
    


    <!-- http://www.w3id.org/eurocodes/ec1990#containsStructuralMember -->


    <owl:ObjectProperty rdf:about="http://www.w3id.org/eurocodes/ec1990#containsStructuralMember">
        <rdfs:subPropertyOf rdf:resource="https://w3id.org/bot#hasElement"/>
        <rdfs:domain rdf:resource="http://www.w3id.org/eurocodes/ec1990#StructuralSystem"/>
        <rdfs:range rdf:resource="http://www.w3id.org/eurocodes/ec1990#StructuralMember"/>
        <rdfs:label xml:lang="en">contains structural member</rdfs:label>
        <skos:definition>Relates a a structural element with the structural system.</skos:definition>
    </owl:ObjectProperty>
    


    <!-- http://www.w3id.org/eurocodes/ec1990#forLimitState -->


    <owl:ObjectProperty rdf:about="http://www.w3id.org/eurocodes/ec1990#forLimitState">
        <rdfs:domain rdf:resource="http://www.w3id.org/eurocodes/ec1990#LimitStateValue"/>
        <rdfs:range rdf:resource="http://www.w3id.org/eurocodes/ec1990#LimitState"/>
        <rdfs:label xml:lang="en">for limit state</rdfs:label>
        <skos:definition>Relates a limit state value with its corresponding limit state.</skos:definition>
    </owl:ObjectProperty>
    


    <!-- http://www.w3id.org/eurocodes/ec1990#hasCharacteristicValue -->


    <owl:ObjectProperty rdf:about="http://www.w3id.org/eurocodes/ec1990#hasCharacteristicValue">
        <rdfs:subPropertyOf rdf:resource="http://qudt.org/3.1.2/schema/qudt/quantityValue"/>
        <rdfs:domain rdf:resource="http://qudt.org/3.1.2/schema/qudt/Quantity"/>
        <rdfs:range rdf:resource="http://www.w3id.org/eurocodes/ec1990#CharacteristicValue"/>
        <rdfs:label xml:lang="en">has characteristic value</rdfs:label>
        <skos:definition>Relates a Quantity  with its Characteristic Value.</skos:definition>
    </owl:ObjectProperty>
    


    <!-- http://www.w3id.org/eurocodes/ec1990#hasDesignValue -->


    <owl:ObjectProperty rdf:about="http://www.w3id.org/eurocodes/ec1990#hasDesignValue">
        <rdfs:subPropertyOf rdf:resource="http://qudt.org/3.1.2/schema/qudt/quantityValue"/>
        <rdfs:domain rdf:resource="http://qudt.org/3.1.2/schema/qudt/Quantity"/>
        <rdfs:range rdf:resource="http://www.w3id.org/eurocodes/ec1990#DesignValue"/>
        <rdfs:label xml:lang="en">has design value</rdfs:label>
        <skos:definition>Relates a Quantity  with its Design Value.</skos:definition>
    </owl:ObjectProperty>
    


    <!-- http://www.w3id.org/eurocodes/ec1990#hasEffect -->


    <owl:ObjectProperty rdf:about="http://www.w3id.org/eurocodes/ec1990#hasEffect">
        <rdfs:domain rdf:resource="http://www.w3id.org/eurocodes/ec1990#StructuralMember"/>
        <rdfs:range rdf:resource="http://www.w3id.org/eurocodes/ec1990#EffectOfAction"/>
        <rdfs:label xml:lang="en">has effect</rdfs:label>
        <skos:definition>Relates a structural member to the effect of action.</skos:definition>
    </owl:ObjectProperty>
    


    <!-- http://www.w3id.org/eurocodes/ec1990#hasGeometricalProperty -->


    <owl:ObjectProperty rdf:about="http://www.w3id.org/eurocodes/ec1990#hasGeometricalProperty">
        <rdfs:domain rdf:resource="http://www.w3id.org/eurocodes/ec1990#StructuralMember"/>
        <rdfs:range rdf:resource="http://www.w3id.org/eurocodes/ec1990#GeometricalProperty"/>
        <rdfs:label xml:lang="en">has geometrical property</rdfs:label>
        <skos:definition>Relates a structural member with its geometrical properties.</skos:definition>
    </owl:ObjectProperty>
    


    <!-- http://www.w3id.org/eurocodes/ec1990#hasLimitStateValue -->


    <owl:ObjectProperty rdf:about="http://www.w3id.org/eurocodes/ec1990#hasLimitStateValue">
        <rdfs:domain rdf:resource="http://www.w3id.org/eurocodes/ec1990#StructuralMember"/>
        <rdfs:range rdf:resource="http://www.w3id.org/eurocodes/ec1990#LimitStateValue"/>
        <rdfs:label xml:lang="en">has limit state value</rdfs:label>
        <skos:definition>Relates a structural member to its capacity for the effect of action.</skos:definition>
    </owl:ObjectProperty>
    


    <!-- http://www.w3id.org/eurocodes/ec1990#hasLowerBoundValue -->


    <owl:ObjectProperty rdf:about="http://www.w3id.org/eurocodes/ec1990#hasLowerBoundValue">
        <rdfs:subPropertyOf rdf:resource="http://qudt.org/3.1.2/schema/qudt/quantityValue"/>
        <rdfs:domain rdf:resource="http://qudt.org/3.1.2/schema/qudt/Quantity"/>
        <rdfs:range rdf:resource="http://www.w3id.org/eurocodes/ec1990#LowerBoundValue"/>
        <rdfs:label xml:lang="en">has lower bound value</rdfs:label>
        <skos:definition>Relates a Quantity  with its Lower Bound Value.</skos:definition>
    </owl:ObjectProperty>
    


    <!-- http://www.w3id.org/eurocodes/ec1990#hasMaterialProperty -->


    <owl:ObjectProperty rdf:about="http://www.w3id.org/eurocodes/ec1990#hasMaterialProperty">
        <rdfs:domain rdf:resource="http://www.w3id.org/eurocodes/ec1990#Material"/>
        <rdfs:range rdf:resource="http://www.w3id.org/eurocodes/ec1990#MaterialProperty"/>
        <rdfs:label xml:lang="en">has material property</rdfs:label>
        <skos:definition>Relates a material with its properties.</skos:definition>
    </owl:ObjectProperty>
    


    <!-- http://www.w3id.org/eurocodes/ec1990#hasMeanValue -->


    <owl:ObjectProperty rdf:about="http://www.w3id.org/eurocodes/ec1990#hasMeanValue">
        <rdfs:subPropertyOf rdf:resource="http://qudt.org/3.1.2/schema/qudt/quantityValue"/>
        <rdfs:domain rdf:resource="http://qudt.org/3.1.2/schema/qudt/Quantity"/>
        <rdfs:range rdf:resource="http://www.w3id.org/eurocodes/ec1990#MeanValue"/>
        <rdfs:label xml:lang="en">has mean value</rdfs:label>
        <skos:definition>Relates a Quantity  with its Mean Value.</skos:definition>
    </owl:ObjectProperty>
    


    <!-- http://www.w3id.org/eurocodes/ec1990#hasNominalValue -->


    <owl:ObjectProperty rdf:about="http://www.w3id.org/eurocodes/ec1990#hasNominalValue">
        <rdfs:subPropertyOf rdf:resource="http://qudt.org/3.1.2/schema/qudt/quantityValue"/>
        <rdfs:domain rdf:resource="http://qudt.org/3.1.2/schema/qudt/Quantity"/>
        <rdfs:range rdf:resource="http://www.w3id.org/eurocodes/ec1990#NominalValue"/>
        <rdfs:label xml:lang="en">has nominal value</rdfs:label>
        <skos:definition>Relates a Quantity  with its Nominal Value.</skos:definition>
    </owl:ObjectProperty>
    


    <!-- http://www.w3id.org/eurocodes/ec1990#hasRepresentativeValue -->


    <owl:ObjectProperty rdf:about="http://www.w3id.org/eurocodes/ec1990#hasRepresentativeValue">
        <rdfs:subPropertyOf rdf:resource="http://qudt.org/3.1.2/schema/qudt/quantityValue"/>
        <rdfs:domain rdf:resource="http://qudt.org/3.1.2/schema/qudt/Quantity"/>
        <rdfs:range rdf:resource="http://www.w3id.org/eurocodes/ec1990#RepresentativeValue"/>
        <rdfs:label xml:lang="en">has representative value</rdfs:label>
        <skos:definition>Relates a Quantity  with its Representative Value.</skos:definition>
    </owl:ObjectProperty>
    


    <!-- http://www.w3id.org/eurocodes/ec1990#hasStructuralMember -->


    <owl:ObjectProperty rdf:about="http://www.w3id.org/eurocodes/ec1990#hasStructuralMember">
        <rdfs:subPropertyOf rdf:resource="https://w3id.org/bot#hasElement"/>
        <rdfs:domain rdf:resource="https://w3id.org/bot#Zone"/>
        <rdfs:range rdf:resource="http://www.w3id.org/eurocodes/ec1990#StructuralMember"/>
        <rdfs:label xml:lang="en">has structural member</rdfs:label>
        <skos:definition>Relates a a structural element with the zone.</skos:definition>
    </owl:ObjectProperty>
    


    <!-- http://www.w3id.org/eurocodes/ec1990#hasStructure -->


    <owl:ObjectProperty rdf:about="http://www.w3id.org/eurocodes/ec1990#hasStructure">
        <rdfs:subPropertyOf rdf:resource="https://w3id.org/bot#hasElement"/>
        <rdfs:domain rdf:resource="http://www.w3id.org/eurocodes/ec1990#ConstructionWork"/>
        <rdfs:range rdf:resource="http://www.w3id.org/eurocodes/ec1990#Structure"/>
        <rdfs:label xml:lang="en">has structure</rdfs:label>
        <skos:definition>Relates a contrution work with the structure.</skos:definition>
    </owl:ObjectProperty>
    


    <!-- http://www.w3id.org/eurocodes/ec1990#hasSystem -->


    <owl:ObjectProperty rdf:about="http://www.w3id.org/eurocodes/ec1990#hasSystem">
        <rdfs:domain rdf:resource="http://www.w3id.org/eurocodes/ec1990#Structure"/>
        <rdfs:range rdf:resource="http://www.w3id.org/eurocodes/ec1990#StructuralSystem"/>
        <rdfs:label xml:lang="en">has system</rdfs:label>
        <skos:definition>Relates a structure with its structural system.</skos:definition>
    </owl:ObjectProperty>
    


    <!-- http://www.w3id.org/eurocodes/ec1990#hasUpperBoundValue -->


    <owl:ObjectProperty rdf:about="http://www.w3id.org/eurocodes/ec1990#hasUpperBoundValue">
        <rdfs:subPropertyOf rdf:resource="http://qudt.org/3.1.2/schema/qudt/quantityValue"/>
        <rdfs:domain rdf:resource="http://qudt.org/3.1.2/schema/qudt/Quantity"/>
        <rdfs:range rdf:resource="http://www.w3id.org/eurocodes/ec1990#UpperBoundValue"/>
        <rdfs:label xml:lang="en">has upper bound value</rdfs:label>
        <skos:definition>Relates a Quantity  with its Upper Bound Value.</skos:definition>
    </owl:ObjectProperty>
    


    <!-- http://www.w3id.org/eurocodes/ec1990#imposesCombination -->


    <owl:ObjectProperty rdf:about="http://www.w3id.org/eurocodes/ec1990#imposesCombination">
        <rdfs:domain rdf:resource="http://www.w3id.org/eurocodes/ec1990#DesignSituation"/>
        <rdfs:range rdf:resource="http://www.w3id.org/eurocodes/ec1990#CombinationOfActions"/>
        <rdfs:label xml:lang="en">imposes combination</rdfs:label>
        <skos:definition>Relates a design situation to the relevant combination.</skos:definition>
    </owl:ObjectProperty>
    


    <!-- http://www.w3id.org/eurocodes/ec1990#isDesignedFor -->


    <owl:ObjectProperty rdf:about="http://www.w3id.org/eurocodes/ec1990#isDesignedFor">
        <rdfs:domain rdf:resource="http://www.w3id.org/eurocodes/ec1990#StructuralMember"/>
        <rdfs:range rdf:resource="http://www.w3id.org/eurocodes/ec1990#DesignSituation"/>
        <rdfs:label xml:lang="en">is designed for</rdfs:label>
        <skos:definition>Relates a structural memeber with the design situation it is designed for.</skos:definition>
    </owl:ObjectProperty>
    


    <!-- http://www.w3id.org/eurocodes/ec1990#isMadeOf -->


    <owl:ObjectProperty rdf:about="http://www.w3id.org/eurocodes/ec1990#isMadeOf">
        <rdfs:domain rdf:resource="http://www.w3id.org/eurocodes/ec1990#StructuralMember"/>
        <rdfs:range rdf:resource="http://www.w3id.org/eurocodes/ec1990#Material"/>
        <rdfs:label xml:lang="en">is made of</rdfs:label>
        <skos:definition>Relates a structural member to the material which it is made of.</skos:definition>
    </owl:ObjectProperty>
    


    <!-- http://www.w3id.org/eurocodes/ec1990#isVerifiedFor -->


    <owl:ObjectProperty rdf:about="http://www.w3id.org/eurocodes/ec1990#isVerifiedFor">
        <rdfs:domain rdf:resource="http://www.w3id.org/eurocodes/ec1990#LimitState"/>
        <rdfs:range rdf:resource="http://www.w3id.org/eurocodes/ec1990#CombinationOfActions"/>
        <rdfs:label xml:lang="en">is verified for</rdfs:label>
        <skos:definition>Relates a limit state to the combination of actions used for its verification.</skos:definition>
    </owl:ObjectProperty>
    


    <!-- http://www.w3id.org/eurocodes/ec1990#requiresVerficationOf -->


    <owl:ObjectProperty rdf:about="http://www.w3id.org/eurocodes/ec1990#requiresVerficationOf">
        <rdfs:domain rdf:resource="http://www.w3id.org/eurocodes/ec1990#DesignSituation"/>
        <rdfs:range rdf:resource="http://www.w3id.org/eurocodes/ec1990#LimitState"/>
        <rdfs:label xml:lang="en">requires verification of</rdfs:label>
        <skos:definition>Relates a limit state to the combination of actions used for its verification.</skos:definition>
    </owl:ObjectProperty>
    


    <!-- http://www.w3id.org/eurocodes/ec1990#usesActionValue -->


    <owl:ObjectProperty rdf:about="http://www.w3id.org/eurocodes/ec1990#usesActionValue">
        <rdfs:domain rdf:resource="http://www.w3id.org/eurocodes/ec1990#CombinationOfActions"/>
        <rdfs:range rdf:resource="http://qudt.org/3.1.2/schema/qudt/QuantityValue"/>
        <rdfs:label xml:lang="en">uses action value</rdfs:label>
        <skos:definition>Relates a combination of actions to the individual actions it contains.</skos:definition>
    </owl:ObjectProperty>
    


    <!-- http://www.w3id.org/eurocodes/ec1990#verifiedAgainstEffect -->


    <owl:ObjectProperty rdf:about="http://www.w3id.org/eurocodes/ec1990#verifiedAgainstEffect">
        <rdfs:domain rdf:resource="http://www.w3id.org/eurocodes/ec1990#LimitStateValue"/>
        <rdfs:range rdf:resource="http://www.w3id.org/eurocodes/ec1990#EffectOfAction"/>
        <rdfs:label xml:lang="en">has limit state value</rdfs:label>
        <skos:definition>Relates a limitstate value with the Action Effect that needs to be verified against.</skos:definition>
    </owl:ObjectProperty>
    


    <!-- 
    ///////////////////////////////////////////////////////////////////////////////////////
    //
    // Data properties
    //
    ///////////////////////////////////////////////////////////////////////////////////////
     -->


    


    <!-- http://www.w3id.org/eurocodes/ec1990#hasCombinationFactor -->


    <owl:DatatypeProperty rdf:about="http://www.w3id.org/eurocodes/ec1990#hasCombinationFactor">
        <rdfs:range rdf:resource="http://www.w3.org/2001/XMLSchema#decimal"/>
        <terms:source>EN 1990:2002, Section 1.5.3.16</terms:source>
        <rdfs:label xml:lang="en">has combination factor</rdfs:label>
        <skos:altLabel>ψ_0</skos:altLabel>
        <skos:definition>Factor for combination value of a variable action used in ultimate limit state verifications.</skos:definition>
    </owl:DatatypeProperty>
    


    <!-- http://www.w3id.org/eurocodes/ec1990#hasDesignWorkingLife -->


    <owl:DatatypeProperty rdf:about="http://www.w3id.org/eurocodes/ec1990#hasDesignWorkingLife">
        <rdfs:domain rdf:resource="http://www.w3id.org/eurocodes/ec1990#Structure"/>
        <rdfs:range rdf:resource="http://www.w3.org/2001/XMLSchema#decimal"/>
        <rdfs:label xml:lang="en">has design working life</rdfs:label>
        <skos:definition>Period during which a structure or structural component is intended to remain functional and to fulfill its performance requirements without major repair or replacement, assuming appropriate maintenance.</skos:definition>
    </owl:DatatypeProperty>
    


    <!-- http://www.w3id.org/eurocodes/ec1990#hasFrequentFactor -->


    <owl:DatatypeProperty rdf:about="http://www.w3id.org/eurocodes/ec1990#hasFrequentFactor">
        <rdfs:range rdf:resource="http://www.w3.org/2001/XMLSchema#decimal"/>
        <terms:source>EN 1990:2002, Section 1.5.3.17</terms:source>
        <rdfs:label xml:lang="en">has frequent factor</rdfs:label>
        <skos:altLabel>ψ_1</skos:altLabel>
        <skos:definition>Factor for frequent value of a variable action, determined so that either the total time within the reference period during which it is exceeded is only a small given part of the reference period, or the frequency of it being exceeded is limited to a given value.</skos:definition>
    </owl:DatatypeProperty>
    


    <!-- http://www.w3id.org/eurocodes/ec1990#hasNationallyDefinedValue -->


    <owl:DatatypeProperty rdf:about="http://www.w3id.org/eurocodes/ec1990#hasNationallyDefinedValue">
        <rdfs:range rdf:resource="http://www.w3.org/2001/XMLSchema#boolean"/>
        <rdfs:label xml:lang="en">has nationally defined value</rdfs:label>
        <skos:definition>Defines whether parameter has specific value defined in NA.</skos:definition>
    </owl:DatatypeProperty>
    


    <!-- http://www.w3id.org/eurocodes/ec1990#hasPartialFactor -->


    <owl:DatatypeProperty rdf:about="http://www.w3id.org/eurocodes/ec1990#hasPartialFactor">
        <rdfs:range rdf:resource="http://www.w3.org/2001/XMLSchema#decimal"/>
        <terms:source>EN 1990:2002, Section 6.3.1</terms:source>
        <rdfs:label xml:lang="en">has partial factor</rdfs:label>
        <skos:altLabel>γ_f</skos:altLabel>
        <skos:definition>Safety factor applied to actions or material properties to account for uncertainties.</skos:definition>
    </owl:DatatypeProperty>
    


    <!-- http://www.w3id.org/eurocodes/ec1990#hasQuasiPermanentFactor -->


    <owl:DatatypeProperty rdf:about="http://www.w3id.org/eurocodes/ec1990#hasQuasiPermanentFactor">
        <rdfs:range rdf:resource="http://www.w3.org/2001/XMLSchema#decimal"/>
        <terms:source>EN 1990:2002, Section 1.5.3.18</terms:source>
        <rdfs:label xml:lang="en">has quasi-permanent factor</rdfs:label>
        <skos:altLabel>ψ_2</skos:altLabel>
        <skos:definition>Factor for quasi-permanent value of a variable action, determined so that the total period of time for which it will be exceeded is a large fraction of the reference period.</skos:definition>
    </owl:DatatypeProperty>
    


    <!-- http://www.w3id.org/eurocodes/ec1990#hasReductionFactor -->


    <owl:DatatypeProperty rdf:about="http://www.w3id.org/eurocodes/ec1990#hasReductionFactor">
        <rdfs:range rdf:resource="http://www.w3.org/2001/XMLSchema#decimal"/>
        <terms:source>EN 1990:2002, Section 6.4.3.2</terms:source>
        <rdfs:label xml:lang="en">has reduction factor</rdfs:label>
        <skos:altLabel>ξ</skos:altLabel>
        <skos:definition>Reduction factor for unfavourable permanent action.</skos:definition>
    </owl:DatatypeProperty>
    


    <!-- http://www.w3id.org/eurocodes/ec1990#isSatisfied -->


    <owl:DatatypeProperty rdf:about="http://www.w3id.org/eurocodes/ec1990#isSatisfied">
        <rdfs:domain rdf:resource="http://www.w3id.org/eurocodes/ec1990#LimitState"/>
        <rdfs:range rdf:resource="http://www.w3.org/2001/XMLSchema#boolean"/>
        <rdfs:label xml:lang="en">is satisfied</rdfs:label>
        <skos:definition>Result of verification of the limit state.</skos:definition>
    </owl:DatatypeProperty>
    


    <!-- 
    ///////////////////////////////////////////////////////////////////////////////////////
    //
    // Classes
    //
    ///////////////////////////////////////////////////////////////////////////////////////
     -->


    


    <!-- http://purl.obolibrary.org/obo/BFO_0000019 -->


    <owl:Class rdf:about="http://purl.obolibrary.org/obo/BFO_0000019"/>
    


    <!-- http://purl.obolibrary.org/obo/BFO_0000040 -->


    <owl:Class rdf:about="http://purl.obolibrary.org/obo/BFO_0000040"/>
    


    <!-- http://purl.obolibrary.org/obo/BFO_0000140 -->


    <owl:Class rdf:about="http://purl.obolibrary.org/obo/BFO_0000140"/>
    


    <!-- http://qudt.org/3.1.2/schema/qudt/Quantity -->


    <owl:Class rdf:about="http://qudt.org/3.1.2/schema/qudt/Quantity"/>
    


    <!-- http://qudt.org/3.1.2/schema/qudt/QuantityValue -->


    <owl:Class rdf:about="http://qudt.org/3.1.2/schema/qudt/QuantityValue"/>
    


    <!-- http://www.w3id.org/eurocodes/ec1990#AccelerationEffect -->


    <owl:Class rdf:about="http://www.w3id.org/eurocodes/ec1990#AccelerationEffect">
        <rdfs:subClassOf rdf:resource="http://www.w3id.org/eurocodes/ec1990#DynamicEffect"/>
        <terms:source>EN 1990:2002, Section 4.1.5(2)</terms:source>
        <rdfs:label xml:lang="en">Acceleration effect</rdfs:label>
        <skos:definition>Effect involving acceleration of the structure or structural members.</skos:definition>
    </owl:Class>
    


    <!-- http://www.w3id.org/eurocodes/ec1990#AccessibleRoofs -->


    <owl:Class rdf:about="http://www.w3id.org/eurocodes/ec1990#AccessibleRoofs">
        <rdfs:subClassOf rdf:resource="http://www.w3id.org/eurocodes/ec1990#EurocodeZone"/>
        <terms:source>EN 1991-1-1:2002 Table 6.9</terms:source>
        <rdfs:label xml:lang="en">Category I - accessible roofs</rdfs:label>
        <skos:definition>Roof accessible with occupancy according to categories A to G</skos:definition>
        <skos:example>Roof used as terraces, gardens, or other occupied spaces</skos:example>
    </owl:Class>
    


    <!-- http://www.w3id.org/eurocodes/ec1990#AccidentalAction -->


    <owl:Class rdf:about="http://www.w3id.org/eurocodes/ec1990#AccidentalAction">
        <rdfs:subClassOf rdf:resource="http://www.w3id.org/eurocodes/ec1990#Action"/>
        <terms:source>EN 1990:2002, Section 1.5.3.5</terms:source>
        <rdfs:label xml:lang="en">Accidental action</rdfs:label>
        <skos:altLabel>A</skos:altLabel>
        <skos:definition>Action, usually of short duration but of significant magnitude, that is unlikely to occur on a given structure during the design working life.</skos:definition>
        <skos:example>explosions, impact from vehicles</skos:example>
    </owl:Class>
    


    <!-- http://www.w3id.org/eurocodes/ec1990#AccidentalCombination -->


    <owl:Class rdf:about="http://www.w3id.org/eurocodes/ec1990#AccidentalCombination">
        <rdfs:subClassOf rdf:resource="http://www.w3id.org/eurocodes/ec1990#ULSCombination"/>
        <owl:disjointWith rdf:resource="http://www.w3id.org/eurocodes/ec1990#FundamentalCombination"/>
        <owl:disjointWith rdf:resource="http://www.w3id.org/eurocodes/ec1990#SeismicCombination"/>
        <terms:source>EN 1990:2002, Section 6.4.3.3</terms:source>
        <rdfs:label xml:lang="en">Accidental combination</rdfs:label>
        <skos:definition>Combination of actions for accidental design situations.</skos:definition>
        <skos:scopeNote>Used for accidental design situations in ULS verifications</skos:scopeNote>
    </owl:Class>
    


    <!-- http://www.w3id.org/eurocodes/ec1990#AccidentalDesignSituation -->


    <owl:Class rdf:about="http://www.w3id.org/eurocodes/ec1990#AccidentalDesignSituation">
        <rdfs:subClassOf rdf:resource="http://www.w3id.org/eurocodes/ec1990#DesignSituation"/>
        <terms:source>EN 1990:2002, Section 1.5.2.5</terms:source>
        <rdfs:label xml:lang="en">Accidental design situation</rdfs:label>
        <skos:definition>Design situation involving exceptional conditions of the structure or its exposure, including fire, explosion, impact or local failure.</skos:definition>
        <skos:example>fire, explosion, impact, local failure</skos:example>
    </owl:Class>
    


    <!-- http://www.w3id.org/eurocodes/ec1990#AccompanyingVariableAction -->


    <owl:Class rdf:about="http://www.w3id.org/eurocodes/ec1990#AccompanyingVariableAction">
        <rdfs:subClassOf rdf:resource="http://www.w3id.org/eurocodes/ec1990#VariableAction"/>
        <owl:disjointWith rdf:resource="http://www.w3id.org/eurocodes/ec1990#LeadingVariableAction"/>
        <terms:source>EN 1990:2002 Section 1.5.3.19)</terms:source>
        <rdfs:label xml:lang="en">Accompanying variable action</rdfs:label>
        <skos:definition>Variable action that accompanies the leading action in a combination.</skos:definition>
    </owl:Class>
    


    <!-- http://www.w3id.org/eurocodes/ec1990#Action -->


    <owl:Class rdf:about="http://www.w3id.org/eurocodes/ec1990#Action">
        <rdfs:subClassOf rdf:resource="http://purl.obolibrary.org/obo/BFO_0000140"/>
        <rdfs:subClassOf rdf:resource="http://qudt.org/3.1.2/schema/qudt/Quantity"/>
        <terms:source>EN 1990:2002, Section 1.5.3.1</terms:source>
        <rdfs:label xml:lang="en">Action</rdfs:label>
        <skos:altLabel>F</skos:altLabel>
        <skos:definition>Set of forces (loads) applied to the structure (direct action) or set of imposed deformations or accelerations caused for example, by temperature changes, moisture variation, uneven settlement or earthquakes (indirect action).</skos:definition>
        <skos:example>dead load, imopsed load, wind load, thermal action</skos:example>
    </owl:Class>
    


    <!-- http://www.w3id.org/eurocodes/ec1990#AngularDeformation -->


    <owl:Class rdf:about="http://www.w3id.org/eurocodes/ec1990#AngularDeformation">
        <rdfs:subClassOf rdf:resource="http://www.w3id.org/eurocodes/ec1990#Deformation"/>
        <owl:disjointWith rdf:resource="http://www.w3id.org/eurocodes/ec1990#LinearDeformation"/>
        <owl:disjointWith rdf:resource="http://www.w3id.org/eurocodes/ec1990#VolumetricDeformation"/>
        <terms:source>EN 1990:2002, Section 1.5.3.2</terms:source>
        <rdfs:label xml:lang="en">Angular deformation</rdfs:label>
        <skos:definition>Deformation involving rotation or angular change in the structure.</skos:definition>
    </owl:Class>
    


    <!-- http://www.w3id.org/eurocodes/ec1990#AreaWithTables -->


    <owl:Class rdf:about="http://www.w3id.org/eurocodes/ec1990#AreaWithTables">
        <rdfs:subClassOf rdf:resource="http://www.w3id.org/eurocodes/ec1990#CongregationArea"/>
        <terms:source>EN 1991-1-1:2002 Table 6.1</terms:source>
        <rdfs:label xml:lang="en">Category C1 - areas with tables</rdfs:label>
        <skos:definition>Area with tables</skos:definition>
        <skos:example>areas in schools, cafés, restaurants, dining halls, reading rooms, receptions</skos:example>
    </owl:Class>
    


    <!-- http://www.w3id.org/eurocodes/ec1990#AreasWithFixedSeats -->


    <owl:Class rdf:about="http://www.w3id.org/eurocodes/ec1990#AreasWithFixedSeats">
        <rdfs:subClassOf rdf:resource="http://www.w3id.org/eurocodes/ec1990#CongregationArea"/>
        <terms:source>EN 1991-1-1:2002 Table 6.1</terms:source>
        <rdfs:label xml:lang="en">Category C2 - areas with fixed seats</rdfs:label>
        <skos:definition>Area with fixed seats</skos:definition>
        <skos:example>areas in churches, theatres or cinemas, conference rooms, lecture halls, assembly halls, waiting rooms, railway waiting rooms</skos:example>
    </owl:Class>
    


    <!-- http://www.w3id.org/eurocodes/ec1990#AreasWithoutObstacle -->


    <owl:Class rdf:about="http://www.w3id.org/eurocodes/ec1990#AreasWithoutObstacle">
        <rdfs:subClassOf rdf:resource="http://www.w3id.org/eurocodes/ec1990#CongregationArea"/>
        <terms:source>EN 1991-1-1:2002 Table 6.1</terms:source>
        <rdfs:label xml:lang="en">Category C3 - areas without obstacles</rdfs:label>
        <skos:definition>Area without obstacles for moving people</skos:definition>
        <skos:example>areas in museums, exhibition rooms, etc. and access areas in public and administration buildings, hotels, hospitals, railway station forecourts</skos:example>
    </owl:Class>
    


    <!-- http://www.w3id.org/eurocodes/ec1990#AxialForce -->


    <owl:Class rdf:about="http://www.w3id.org/eurocodes/ec1990#AxialForce">
        <rdfs:subClassOf rdf:resource="http://www.w3id.org/eurocodes/ec1990#InternalForce"/>
        <terms:source>EN 1990:2002, Section 1.5.3.2</terms:source>
        <rdfs:label xml:lang="en">Axial force</rdfs:label>
        <skos:altLabel>N</skos:altLabel>
        <skos:definition>Internal force acting along the axis of structural members.</skos:definition>
    </owl:Class>
    


    <!-- http://www.w3id.org/eurocodes/ec1990#BendingMoment -->


    <owl:Class rdf:about="http://www.w3id.org/eurocodes/ec1990#BendingMoment">
        <rdfs:subClassOf rdf:resource="http://www.w3id.org/eurocodes/ec1990#InternalForce"/>
        <terms:source>EN 1990:2002, Section 1.5.3.2</terms:source>
        <rdfs:label xml:lang="en">Bending moment</rdfs:label>
        <skos:altLabel>M</skos:altLabel>
        <skos:definition>Internal moment causing bending in structural members.</skos:definition>
    </owl:Class>
    


    <!-- http://www.w3id.org/eurocodes/ec1990#BendingMomentResistance -->


    <owl:Class rdf:about="http://www.w3id.org/eurocodes/ec1990#BendingMomentResistance">
        <rdfs:subClassOf rdf:resource="http://www.w3id.org/eurocodes/ec1990#Resistance"/>
        <rdfs:label xml:lang="en">Bending moment resistance</rdfs:label>
        <skos:altLabel>M_Rd</skos:altLabel>
        <skos:definition>Design value of the maximum bending moment that a structural cross-section can safely resist without failure.</skos:definition>
    </owl:Class>
    


    <!-- http://www.w3id.org/eurocodes/ec1990#Building -->


    <owl:Class rdf:about="http://www.w3id.org/eurocodes/ec1990#Building">
        <rdfs:subClassOf rdf:resource="http://www.w3id.org/eurocodes/ec1990#ConstructionWork"/>
    </owl:Class>
    


    <!-- http://www.w3id.org/eurocodes/ec1990#CharacteristicCombination -->


    <owl:Class rdf:about="http://www.w3id.org/eurocodes/ec1990#CharacteristicCombination">
        <rdfs:subClassOf rdf:resource="http://www.w3id.org/eurocodes/ec1990#SLSCombination"/>
        <owl:disjointWith rdf:resource="http://www.w3id.org/eurocodes/ec1990#FrequentCombination"/>
        <owl:disjointWith rdf:resource="http://www.w3id.org/eurocodes/ec1990#QuasiPermanentCombination"/>
        <terms:source>EN 1990:2002, Section 6.5.3(2)a</terms:source>
        <rdfs:label xml:lang="en">Characteristic combination</rdfs:label>
        <skos:definition>Serviceability combination normally used for irreversible limit states.</skos:definition>
        <skos:scopeNote>Used for irreversible serviceability limit state verifications</skos:scopeNote>
    </owl:Class>
    


    <!-- http://www.w3id.org/eurocodes/ec1990#CharacteristicValue -->


    <owl:Class rdf:about="http://www.w3id.org/eurocodes/ec1990#CharacteristicValue">
        <rdfs:subClassOf rdf:resource="http://qudt.org/3.1.2/schema/qudt/QuantityValue"/>
        <rdfs:label xml:lang="en">Characteristic value</rdfs:label>
        <skos:definition>A statistically defined value of a physical quantity with a specified probability of non-exceedance.</skos:definition>
    </owl:Class>
    


    <!-- http://www.w3id.org/eurocodes/ec1990#CivilEngineeringWork -->


    <owl:Class rdf:about="http://www.w3id.org/eurocodes/ec1990#CivilEngineeringWork">
        <rdfs:subClassOf rdf:resource="http://www.w3id.org/eurocodes/ec1990#ConstructionWork"/>
        <terms:source>EN 1990:2002, Section 1.5.1.2</terms:source>
        <rdfs:label xml:lang="en">Civil engineering work</rdfs:label>
        <skos:definition>Type of construction work for civil engineering purposes such as bridges, retaining walls, etc.</skos:definition>
        <skos:example>bridge, retaining wall, tunnel</skos:example>
    </owl:Class>
    


    <!-- http://www.w3id.org/eurocodes/ec1990#CombinationOfActions -->


    <owl:Class rdf:about="http://www.w3id.org/eurocodes/ec1990#CombinationOfActions">
        <rdfs:subClassOf rdf:resource="http://purl.obolibrary.org/obo/BFO_0000140"/>
        <terms:source>EN 1990:2002, Section 1.5.3.22</terms:source>
        <rdfs:label xml:lang="en">Combination of actions</rdfs:label>
        <skos:definition>Set of design values used for the verification of the structural reliability for a limit state under the simultaneous influence of different actions.</skos:definition>
    </owl:Class>
    


    <!-- http://www.w3id.org/eurocodes/ec1990#CompressiveStrength -->


    <owl:Class rdf:about="http://www.w3id.org/eurocodes/ec1990#CompressiveStrength">
        <rdfs:subClassOf rdf:resource="http://www.w3id.org/eurocodes/ec1990#MaterialProperty"/>
        <rdfs:label xml:lang="en">Compressive strength</rdfs:label>
        <skos:definition>Compressive strength of a material.</skos:definition>
    </owl:Class>
    


    <!-- http://www.w3id.org/eurocodes/ec1990#Concrete -->


    <owl:Class rdf:about="http://www.w3id.org/eurocodes/ec1990#Concrete">
        <rdfs:subClassOf rdf:resource="http://www.w3id.org/eurocodes/ec1990#Material"/>
        <rdfs:label xml:lang="en">Concrete</rdfs:label>
        <skos:definition>A composite material consisting of a mixture of cement, water, aggregates (coarse and fine), and, where appropriate, admixtures and additions, which develops its strength by hydration of the cement. </skos:definition>
    </owl:Class>
    


    <!-- http://www.w3id.org/eurocodes/ec1990#CongregationArea -->


    <owl:Class rdf:about="http://www.w3id.org/eurocodes/ec1990#CongregationArea">
        <rdfs:subClassOf rdf:resource="http://www.w3id.org/eurocodes/ec1990#EurocodeZone"/>
        <terms:source>EN 1991-1-1:2002 Table 6.1</terms:source>
        <rdfs:label xml:lang="en">Category C - congregation areas</rdfs:label>
        <skos:definition>Area where people may congregate (except areas under category A, B, and D)</skos:definition>
    </owl:Class>
    


    <!-- http://www.w3id.org/eurocodes/ec1990#ConstructionWork -->


    <owl:Class rdf:about="http://www.w3id.org/eurocodes/ec1990#ConstructionWork">
        <rdfs:subClassOf rdf:resource="http://purl.obolibrary.org/obo/BFO_0000040"/>
        <terms:source>EN 1990:2002, Section 1.5.1.1</terms:source>
        <rdfs:label xml:lang="en">Construction works</rdfs:label>
        <skos:definition>Everything that is constructed or results from construction operations. The term covers both building and civil engineering works comprising structural, non-structural and geotechnical elements.</skos:definition>
        <skos:example>building, bridge, nuclea power plant</skos:example>
    </owl:Class>
    


    <!-- http://www.w3id.org/eurocodes/ec1990#CreepEffect -->


    <owl:Class rdf:about="http://www.w3id.org/eurocodes/ec1990#CreepEffect">
        <rdfs:subClassOf rdf:resource="http://www.w3id.org/eurocodes/ec1990#TimeDependentEffect"/>
        <rdfs:label xml:lang="en">Creep effect</rdfs:label>
        <skos:definition>Long-term deformation effect due to sustained loading.</skos:definition>
    </owl:Class>
    


    <!-- http://www.w3id.org/eurocodes/ec1990#DeadLoad -->


    <owl:Class rdf:about="http://www.w3id.org/eurocodes/ec1990#DeadLoad">
        <rdfs:subClassOf rdf:resource="http://www.w3id.org/eurocodes/ec1990#PermanentAction"/>
        <terms:source>EN 1991-1-1:2002</terms:source>
        <rdfs:label xml:lang="en">Dead load</rdfs:label>
        <skos:definition>.</skos:definition>
    </owl:Class>
    


    <!-- http://www.w3id.org/eurocodes/ec1990#Deflection -->


    <owl:Class rdf:about="http://www.w3id.org/eurocodes/ec1990#Deflection">
        <rdfs:subClassOf rdf:resource="http://www.w3id.org/eurocodes/ec1990#LinearDeformation"/>
        <terms:source>EN 1990:2002, Section 1.6</terms:source>
        <rdfs:label xml:lang="en">Deflection</rdfs:label>
        <skos:altLabel>w</skos:altLabel>
        <skos:definition>Vertical deflction of a structural member.</skos:definition>
    </owl:Class>
    


    <!-- http://www.w3id.org/eurocodes/ec1990#Deformation -->


    <owl:Class rdf:about="http://www.w3id.org/eurocodes/ec1990#Deformation">
        <rdfs:subClassOf rdf:resource="http://www.w3id.org/eurocodes/ec1990#DeformationEffect"/>
        <terms:source>EN 1990:2002, Section 1.5.3.2</terms:source>
        <rdfs:label xml:lang="en">Deformation</rdfs:label>
        <skos:definition>Change in shape or size of a structure or structural member due to actions.</skos:definition>
    </owl:Class>
    


    <!-- http://www.w3id.org/eurocodes/ec1990#DeformationEffect -->


    <owl:Class rdf:about="http://www.w3id.org/eurocodes/ec1990#DeformationEffect">
        <rdfs:subClassOf rdf:resource="http://www.w3id.org/eurocodes/ec1990#EffectOfAction"/>
        <rdfs:label xml:lang="en">Deformation effect</rdfs:label>
        <skos:definition>Effect of actions in the form of deformations of the structure or structural members.</skos:definition>
    </owl:Class>
    


    <!-- http://www.w3id.org/eurocodes/ec1990#Density -->


    <owl:Class rdf:about="http://www.w3id.org/eurocodes/ec1990#Density">
        <rdfs:subClassOf rdf:resource="http://www.w3id.org/eurocodes/ec1990#MaterialProperty"/>
        <rdfs:label xml:lang="en">Density</rdfs:label>
        <skos:definition>Mass per unit volume of a material.</skos:definition>
    </owl:Class>
    


    <!-- http://www.w3id.org/eurocodes/ec1990#DepartmentStore -->


    <owl:Class rdf:about="http://www.w3id.org/eurocodes/ec1990#DepartmentStore">
        <rdfs:subClassOf rdf:resource="http://www.w3id.org/eurocodes/ec1990#ShoppingAreas"/>
        <terms:source>EN 1991-1-1:2002 Table 6.1</terms:source>
        <rdfs:label xml:lang="en">Category D2 - department stores</rdfs:label>
        <skos:definition>Area in department stores</skos:definition>
        <skos:example>department stores</skos:example>
    </owl:Class>
    


    <!-- http://www.w3id.org/eurocodes/ec1990#DesignAction -->


    <owl:Class rdf:about="http://www.w3id.org/eurocodes/ec1990#DesignAction">
        <rdfs:subClassOf rdf:resource="http://www.w3id.org/eurocodes/ec1990#Action"/>
        <owl:disjointWith rdf:resource="http://www.w3id.org/eurocodes/ec1990#RepresentativeAction"/>
        <terms:source>EN 1990:2002, Section 1.5.3.21</terms:source>
        <rdfs:label xml:lang="en">Design action</rdfs:label>
        <skos:definition>Value ofan action used for limit state verification. A design valueo is btained by multiplying the representative value by the partial factor.</skos:definition>
    </owl:Class>
    


    <!-- http://www.w3id.org/eurocodes/ec1990#DesignSituation -->


    <owl:Class rdf:about="http://www.w3id.org/eurocodes/ec1990#DesignSituation">
        <terms:source>EN 1990:2002, Section 1.5.2.2</terms:source>
        <rdfs:label xml:lang="en">Design situation</rdfs:label>
        <skos:definition>Sets of physical conditions representing the real conditions occurring during a certain time interval for which the design will demonstrate that relevant limit states are not exceeded.</skos:definition>
    </owl:Class>
    


    <!-- http://www.w3id.org/eurocodes/ec1990#DesignValue -->


    <owl:Class rdf:about="http://www.w3id.org/eurocodes/ec1990#DesignValue">
        <rdfs:subClassOf rdf:resource="http://qudt.org/3.1.2/schema/qudt/QuantityValue"/>
        <rdfs:label xml:lang="en">Design value</rdfs:label>
        <skos:definition>A value used in structural design verification, derived from a representative value (typically characteristic) through application of partial safety factors.</skos:definition>
    </owl:Class>
    


    <!-- http://www.w3id.org/eurocodes/ec1990#DirectAction -->


    <owl:Class rdf:about="http://www.w3id.org/eurocodes/ec1990#DirectAction">
        <rdfs:subClassOf rdf:resource="http://www.w3id.org/eurocodes/ec1990#Action"/>
        <owl:disjointWith rdf:resource="http://www.w3id.org/eurocodes/ec1990#IndirectAction"/>
        <terms:source>EN 1990:2002, Section 1.5.3.1 a)</terms:source>
        <rdfs:label xml:lang="en">Direct action</rdfs:label>
        <skos:definition>Set of forces (loads) applied to the structure.</skos:definition>
    </owl:Class>
    


    <!-- http://www.w3id.org/eurocodes/ec1990#Displacement -->


    <owl:Class rdf:about="http://www.w3id.org/eurocodes/ec1990#Displacement">
        <rdfs:subClassOf rdf:resource="http://www.w3id.org/eurocodes/ec1990#LinearDeformation"/>
        <terms:source>EN 1990:2002, Section 1.6</terms:source>
        <rdfs:label xml:lang="en">Displacement</rdfs:label>
        <skos:altLabel>u</skos:altLabel>
        <skos:definition>Horizontal displacement of a structure or structural member.</skos:definition>
    </owl:Class>
    


    <!-- http://www.w3id.org/eurocodes/ec1990#DynamicAction -->


    <owl:Class rdf:about="http://www.w3id.org/eurocodes/ec1990#DynamicAction">
        <rdfs:subClassOf rdf:resource="http://www.w3id.org/eurocodes/ec1990#Action"/>
        <owl:disjointWith rdf:resource="http://www.w3id.org/eurocodes/ec1990#StaticAction"/>
        <terms:source>EN 1990:2002, Section 1.5.3.12</terms:source>
        <rdfs:label xml:lang="en">Dynamic action</rdfs:label>
        <skos:definition>Action that causes significant acceleration of the structure or structural members.</skos:definition>
    </owl:Class>
    


    <!-- http://www.w3id.org/eurocodes/ec1990#DynamicEffect -->


    <owl:Class rdf:about="http://www.w3id.org/eurocodes/ec1990#DynamicEffect">
        <rdfs:subClassOf rdf:resource="http://www.w3id.org/eurocodes/ec1990#EffectOfAction"/>
        <rdfs:label xml:lang="en">Dynamic effect</rdfs:label>
        <skos:definition>Effect of actions involving dynamic response, acceleration, or vibration.</skos:definition>
    </owl:Class>
    


    <!-- http://www.w3id.org/eurocodes/ec1990#EffectOfAction -->


    <owl:Class rdf:about="http://www.w3id.org/eurocodes/ec1990#EffectOfAction">
        <rdfs:subClassOf rdf:resource="http://purl.obolibrary.org/obo/BFO_0000140"/>
        <rdfs:subClassOf rdf:resource="http://qudt.org/3.1.2/schema/qudt/Quantity"/>
        <terms:source>EN 1990:2002, Section 1.5.3.2</terms:source>
        <rdfs:label xml:lang="en">Effect of action</rdfs:label>
        <skos:altLabel>E</skos:altLabel>
        <skos:definition>Effect of actions on structural members (e.g. internal force, moment, stress, strain) or on the whole structure (e.g. deflection, rotation).</skos:definition>
        <skos:editorialNote>Effects of actions can be calculated through structural analysis and must be compared against resistance for verification</skos:editorialNote>
        <skos:example>internal force, moment, stress, strain, deflection, rotation</skos:example>
    </owl:Class>
    


    <!-- http://www.w3id.org/eurocodes/ec1990#EurocodeZone -->


    <owl:Class rdf:about="http://www.w3id.org/eurocodes/ec1990#EurocodeZone">
        <rdfs:subClassOf rdf:resource="http://purl.obolibrary.org/obo/BFO_0000040"/>
        <rdfs:subClassOf rdf:resource="https://w3id.org/bot#Zone"/>
        <terms:source>EN 1991-1-1:2002 Table 6.1</terms:source>
        <rdfs:label xml:lang="en">Eurocode zone</rdfs:label>
        <skos:definition>A space classified according to EN 1991-1-1 usage categories</skos:definition>
    </owl:Class>
    


    <!-- http://www.w3id.org/eurocodes/ec1990#FatigueAction -->


    <owl:Class rdf:about="http://www.w3id.org/eurocodes/ec1990#FatigueAction">
        <rdfs:subClassOf rdf:resource="http://www.w3id.org/eurocodes/ec1990#Action"/>
        <terms:source>EN 1990:2002, Section 1.5.3.7</terms:source>
        <rdfs:label xml:lang="en">Fatigue action</rdfs:label>
        <skos:definition>Repeated or fluctuating mechanical action applied over time, which may cause failure even if the individual stress cycles are below the material&apos;s static strength.</skos:definition>
    </owl:Class>
    


    <!-- http://www.w3id.org/eurocodes/ec1990#FatigueEffect -->


    <owl:Class rdf:about="http://www.w3id.org/eurocodes/ec1990#FatigueEffect">
        <rdfs:subClassOf rdf:resource="http://www.w3id.org/eurocodes/ec1990#TimeDependentEffect"/>
        <terms:source>EN 1990:2002, Section 3.1(5)</terms:source>
        <rdfs:label xml:lang="en">Fatigue effect</rdfs:label>
        <skos:definition>Progressive damage effect due to repeated loading cycles.</skos:definition>
    </owl:Class>
    


    <!-- http://www.w3id.org/eurocodes/ec1990#FavourableAction -->


    <owl:Class rdf:about="http://www.w3id.org/eurocodes/ec1990#FavourableAction">
        <rdfs:subClassOf rdf:resource="http://www.w3id.org/eurocodes/ec1990#Action"/>
        <owl:disjointWith rdf:resource="http://www.w3id.org/eurocodes/ec1990#UnfavourableAction"/>
        <terms:source>EN 1990:2002, Section 6.3.2(3)P</terms:source>
        <rdfs:label xml:lang="en">Favourable action</rdfs:label>
        <skos:definition>Action that reduces the effect of other actions on a structure, or otherwise contributes to structural safety.</skos:definition>
    </owl:Class>
    


    <!-- http://www.w3id.org/eurocodes/ec1990#FixedAction -->


    <owl:Class rdf:about="http://www.w3id.org/eurocodes/ec1990#FixedAction">
        <rdfs:subClassOf rdf:resource="http://www.w3id.org/eurocodes/ec1990#Action"/>
        <owl:disjointWith rdf:resource="http://www.w3id.org/eurocodes/ec1990#FreeAction"/>
        <terms:source>EN 1990:2002, Section 1.5.3.8</terms:source>
        <rdfs:label xml:lang="en">Fixed action</rdfs:label>
        <skos:definition>Action that has a fixed distribution and position over the structure or structural member such that the magnitude and direction of the action are determined unambiguously for the whole structure.</skos:definition>
        <skos:example>Stored goods in a defined storage area with no alternative placement</skos:example>
    </owl:Class>
    


    <!-- http://www.w3id.org/eurocodes/ec1990#FreeAction -->


    <owl:Class rdf:about="http://www.w3id.org/eurocodes/ec1990#FreeAction">
        <rdfs:subClassOf rdf:resource="http://www.w3id.org/eurocodes/ec1990#Action"/>
        <terms:source>EN 1990:2002, Section 1.5.3.9</terms:source>
        <rdfs:label xml:lang="en">Free action</rdfs:label>
        <skos:definition>Action that may have various spatial distributions over the structure.</skos:definition>
        <skos:example>Imposed floor load on individual rooms of a multi-storey building</skos:example>
    </owl:Class>
    


    <!-- http://www.w3id.org/eurocodes/ec1990#FrequentCombination -->


    <owl:Class rdf:about="http://www.w3id.org/eurocodes/ec1990#FrequentCombination">
        <rdfs:subClassOf rdf:resource="http://www.w3id.org/eurocodes/ec1990#SLSCombination"/>
        <owl:disjointWith rdf:resource="http://www.w3id.org/eurocodes/ec1990#QuasiPermanentCombination"/>
        <terms:source>EN 1990:2002, Section 6.5.3(2)b</terms:source>
        <rdfs:label xml:lang="en">Frequent combination</rdfs:label>
        <skos:definition>Serviceability combination normally used for reversible limit states.</skos:definition>
        <skos:scopeNote>Used for reversible serviceability limit state verifications</skos:scopeNote>
    </owl:Class>
    


    <!-- http://www.w3id.org/eurocodes/ec1990#FundamentalCombination -->


    <owl:Class rdf:about="http://www.w3id.org/eurocodes/ec1990#FundamentalCombination">
        <rdfs:subClassOf rdf:resource="http://www.w3id.org/eurocodes/ec1990#ULSCombination"/>
        <owl:disjointWith rdf:resource="http://www.w3id.org/eurocodes/ec1990#SeismicCombination"/>
        <terms:source>EN 1990:2002, Section 6.4.3.2</terms:source>
        <rdfs:label xml:lang="en">Fundamental combination</rdfs:label>
        <skos:definition>Combination of actions for persistent or transient design situations.</skos:definition>
        <skos:scopeNote>Used for persistent and transient design situations in ULS verifications</skos:scopeNote>
    </owl:Class>
    


    <!-- http://www.w3id.org/eurocodes/ec1990#GeneralRetailShops -->


    <owl:Class rdf:about="http://www.w3id.org/eurocodes/ec1990#GeneralRetailShops">
        <rdfs:subClassOf rdf:resource="http://www.w3id.org/eurocodes/ec1990#ShoppingAreas"/>
        <terms:source>EN 1991-1-1:2002 Table 6.1</terms:source>
        <rdfs:label xml:lang="en">Category D1 - general retail shops</rdfs:label>
        <skos:definition>Area in general retail shops</skos:definition>
        <skos:example>general retail shops</skos:example>
    </owl:Class>
    


    <!-- http://www.w3id.org/eurocodes/ec1990#GeometricalProperty -->


    <owl:Class rdf:about="http://www.w3id.org/eurocodes/ec1990#GeometricalProperty">
        <rdfs:subClassOf rdf:resource="http://purl.obolibrary.org/obo/BFO_0000019"/>
        <rdfs:subClassOf rdf:resource="http://qudt.org/3.1.2/schema/qudt/Quantity"/>
        <terms:source>EN 1990:2002, Section 4.3</terms:source>
        <rdfs:label xml:lang="en">Geometrical data</rdfs:label>
        <skos:definition>Geometrical properties and dimensions of structural elements.</skos:definition>
    </owl:Class>
    


    <!-- http://www.w3id.org/eurocodes/ec1990#GeotechnicalAction -->


    <owl:Class rdf:about="http://www.w3id.org/eurocodes/ec1990#GeotechnicalAction">
        <rdfs:subClassOf rdf:resource="http://www.w3id.org/eurocodes/ec1990#Action"/>
        <terms:source>EN 1990:2002, Section 1.5.3.7</terms:source>
        <rdfs:label xml:lang="en">Geotechnical action</rdfs:label>
        <skos:definition>Action transmitted to the structure by the ground, fill or groundwater.</skos:definition>
    </owl:Class>
    


    <!-- http://www.w3id.org/eurocodes/ec1990#HelicopterLandingAreas -->


    <owl:Class rdf:about="http://www.w3id.org/eurocodes/ec1990#HelicopterLandingAreas">
        <rdfs:subClassOf rdf:resource="http://www.w3id.org/eurocodes/ec1990#EurocodeZone"/>
        <terms:source>EN 1991-1-1:2002 Table 6.9</terms:source>
        <rdfs:label xml:lang="en">Category K - helicopter landing areas</rdfs:label>
        <skos:definition>Roof accessible for special services, such as helicopter landing areas</skos:definition>
        <skos:example>helicopter landing pads on roofs</skos:example>
    </owl:Class>
    


    <!-- http://www.w3id.org/eurocodes/ec1990#ImposedLoad -->


    <owl:Class rdf:about="http://www.w3id.org/eurocodes/ec1990#ImposedLoad">
        <rdfs:subClassOf rdf:resource="http://www.w3id.org/eurocodes/ec1990#VariableAction"/>
        <owl:disjointWith rdf:resource="http://www.w3id.org/eurocodes/ec1990#SnowLoad"/>
        <owl:disjointWith rdf:resource="http://www.w3id.org/eurocodes/ec1990#ThermalAction"/>
        <owl:disjointWith rdf:resource="http://www.w3id.org/eurocodes/ec1990#WindAction"/>
        <terms:source>EN 1991-1-1:2002</terms:source>
        <rdfs:label xml:lang="en">Imposed load</rdfs:label>
        <skos:definition>Loads that is not permanent and arise from the intended use or occupancy of the structure.</skos:definition>
    </owl:Class>
    


    <!-- http://www.w3id.org/eurocodes/ec1990#IndirectAction -->


    <owl:Class rdf:about="http://www.w3id.org/eurocodes/ec1990#IndirectAction">
        <rdfs:subClassOf rdf:resource="http://www.w3id.org/eurocodes/ec1990#Action"/>
        <terms:source>EN 1990:2002, Section 1.5.3.1 b)</terms:source>
        <rdfs:label xml:lang="en">Indirect action</rdfs:label>
        <skos:definition>Set of imposed deformations or accelerations caused for example, by temperature changes, moisture variation, uneven settlement or earthquakes.</skos:definition>
    </owl:Class>
    


    <!-- http://www.w3id.org/eurocodes/ec1990#IndustrialUse -->


    <owl:Class rdf:about="http://www.w3id.org/eurocodes/ec1990#IndustrialUse">
        <rdfs:subClassOf rdf:resource="http://www.w3id.org/eurocodes/ec1990#IndustrialandStorage"/>
        <terms:source>EN 1991-1-1:2002 Table 6.3</terms:source>
        <rdfs:label xml:lang="en">Category E2 - industrial use</rdfs:label>
        <skos:definition>Industrial use area</skos:definition>
        <skos:example>industrial facilities: plant rooms, workshops</skos:example>
    </owl:Class>
    


    <!-- http://www.w3id.org/eurocodes/ec1990#IndustrialandStorage -->


    <owl:Class rdf:about="http://www.w3id.org/eurocodes/ec1990#IndustrialandStorage">
        <rdfs:subClassOf rdf:resource="http://www.w3id.org/eurocodes/ec1990#EurocodeZone"/>
        <terms:source>EN 1991-1-1:2002 Table 6.3</terms:source>
        <rdfs:label xml:lang="en">Category E - storage and industrial</rdfs:label>
        <skos:definition>Storage and industrial area</skos:definition>
    </owl:Class>
    


    <!-- http://www.w3id.org/eurocodes/ec1990#InternalForce -->


    <owl:Class rdf:about="http://www.w3id.org/eurocodes/ec1990#InternalForce">
        <rdfs:subClassOf rdf:resource="http://www.w3id.org/eurocodes/ec1990#MechanicalEffect"/>
        <terms:source>EN 1990:2002, Section 1.5.3.2</terms:source>
        <rdfs:label xml:lang="en">Internal force</rdfs:label>
        <skos:definition>Effect of actions in the form of internal forces in structural members.</skos:definition>
    </owl:Class>
    


    <!-- http://www.w3id.org/eurocodes/ec1990#LargeCrowdsAreas -->


    <owl:Class rdf:about="http://www.w3id.org/eurocodes/ec1990#LargeCrowdsAreas">
        <rdfs:subClassOf rdf:resource="http://www.w3id.org/eurocodes/ec1990#CongregationArea"/>
        <terms:source>EN 1991-1-1:2002 Table 6.1</terms:source>
        <rdfs:label xml:lang="en">Category C5 - large crowds areas</rdfs:label>
        <skos:definition>Area susceptible to large crowds</skos:definition>
        <skos:example>buildings for public events like concert halls, sports halls including stands, terraces and access areas and railway platforms</skos:example>
    </owl:Class>
    


    <!-- http://www.w3id.org/eurocodes/ec1990#LeadingVariableAction -->


    <owl:Class rdf:about="http://www.w3id.org/eurocodes/ec1990#LeadingVariableAction">
        <rdfs:subClassOf rdf:resource="http://www.w3id.org/eurocodes/ec1990#VariableAction"/>
        <terms:source>EN 1990:2002 Section 6.4.3.1(2)</terms:source>
        <rdfs:label xml:lang="en">Leading variable action</rdfs:label>
        <skos:definition>Variable action that, in a particular combination of actions, has the most significant effect on the design outcome and is considered as the primary representative of the variable actions in that combination.</skos:definition>
    </owl:Class>
    


    <!-- http://www.w3id.org/eurocodes/ec1990#LightVehicleTraffic -->


    <owl:Class rdf:about="http://www.w3id.org/eurocodes/ec1990#LightVehicleTraffic">
        <rdfs:subClassOf rdf:resource="http://www.w3id.org/eurocodes/ec1990#EurocodeZone"/>
        <terms:source>EN 1991-1-1:2002 Table 6.7</terms:source>
        <rdfs:label xml:lang="en">Category F - light vehicle traffic</rdfs:label>
        <skos:definition>Traffic and parking area for light vehicles (≤ 30 kN gross vehicle weight and ≤ 8 seats not including driver)</skos:definition>
        <skos:example>garages, parking areas, parking halls</skos:example>
    </owl:Class>
    


    <!-- http://www.w3id.org/eurocodes/ec1990#LimitState -->


    <owl:Class rdf:about="http://www.w3id.org/eurocodes/ec1990#LimitState">
        <terms:source>EN 1990:2002, Section 1.5.2.12</terms:source>
        <rdfs:label xml:lang="en">Limit state</rdfs:label>
        <skos:definition>State beyond which the structure no longer fulfils the relevant design criteria.</skos:definition>
        <skos:editorialNote>Limit states define critical conditions that must not be exceeded to ensure structural safety and serviceability</skos:editorialNote>
    </owl:Class>
    


    <!-- http://www.w3id.org/eurocodes/ec1990#LimitStateValue -->


    <owl:Class rdf:about="http://www.w3id.org/eurocodes/ec1990#LimitStateValue">
        <rdfs:subClassOf rdf:resource="http://qudt.org/3.1.2/schema/qudt/Quantity"/>
        <rdfs:label xml:lang="en">Limit state value</rdfs:label>
        <skos:definition>Design resistance or serviceability criterion used for verificatinon of a limit state.</skos:definition>
    </owl:Class>
    


    <!-- http://www.w3id.org/eurocodes/ec1990#LimitingServicabilityCriterion -->


    <owl:Class rdf:about="http://www.w3id.org/eurocodes/ec1990#LimitingServicabilityCriterion">
        <rdfs:subClassOf rdf:resource="http://www.w3id.org/eurocodes/ec1990#LimitStateValue"/>
        <terms:source>EN 1990:2002, Section 6.5.1</terms:source>
        <rdfs:label xml:lang="en">Limiting serviceability criterion</rdfs:label>
        <skos:definition>Limiting design value of the relevant serviceability criterion.</skos:definition>
        <skos:example>allowable deflection, allowable crack width</skos:example>
    </owl:Class>
    


    <!-- http://www.w3id.org/eurocodes/ec1990#LinearDeformation -->


    <owl:Class rdf:about="http://www.w3id.org/eurocodes/ec1990#LinearDeformation">
        <rdfs:subClassOf rdf:resource="http://www.w3id.org/eurocodes/ec1990#Deformation"/>
        <owl:disjointWith rdf:resource="http://www.w3id.org/eurocodes/ec1990#VolumetricDeformation"/>
        <rdfs:label xml:lang="en">Linear deformation</rdfs:label>
        <skos:definition>Deformation involving linear displacement of points in the structure.</skos:definition>
    </owl:Class>
    


    <!-- http://www.w3id.org/eurocodes/ec1990#LowerBoundValue -->


    <owl:Class rdf:about="http://www.w3id.org/eurocodes/ec1990#LowerBoundValue">
        <rdfs:subClassOf rdf:resource="http://qudt.org/3.1.2/schema/qudt/QuantityValue"/>
        <rdfs:label xml:lang="en">Lower bound value</rdfs:label>
        <skos:definition>A conservative or code-specified minimum value of a physical quantity, used to ensure safety under unfavorable conditions.</skos:definition>
    </owl:Class>
    


    <!-- http://www.w3id.org/eurocodes/ec1990#Material -->


    <owl:Class rdf:about="http://www.w3id.org/eurocodes/ec1990#Material">
        <terms:source>EN 1990:2002, Section 1.5.1.3</terms:source>
        <rdfs:label xml:lang="en">Material</rdfs:label>
        <skos:definition>Indication of the principal structural material.</skos:definition>
    </owl:Class>
    


    <!-- http://www.w3id.org/eurocodes/ec1990#MaterialProperty -->


    <owl:Class rdf:about="http://www.w3id.org/eurocodes/ec1990#MaterialProperty">
        <rdfs:subClassOf rdf:resource="http://purl.obolibrary.org/obo/BFO_0000019"/>
        <rdfs:subClassOf rdf:resource="http://qudt.org/3.1.2/schema/qudt/Quantity"/>
        <terms:source>EN 1990:2002, Section 4.2</terms:source>
        <rdfs:label xml:lang="en">Material property</rdfs:label>
        <skos:definition>Physical or mechanical property of construction materials.</skos:definition>
    </owl:Class>
    


    <!-- http://www.w3id.org/eurocodes/ec1990#MeanValue -->


    <owl:Class rdf:about="http://www.w3id.org/eurocodes/ec1990#MeanValue">
        <rdfs:subClassOf rdf:resource="http://qudt.org/3.1.2/schema/qudt/QuantityValue"/>
        <rdfs:label xml:lang="en">Mean value</rdfs:label>
        <skos:definition>Arithmetic average of a set of observations; used to represent the expected or central value of a physical quantity in structural design.</skos:definition>
    </owl:Class>
    


    <!-- http://www.w3id.org/eurocodes/ec1990#MechanicalEffect -->


    <owl:Class rdf:about="http://www.w3id.org/eurocodes/ec1990#MechanicalEffect">
        <rdfs:subClassOf rdf:resource="http://www.w3id.org/eurocodes/ec1990#EffectOfAction"/>
        <rdfs:label xml:lang="en">Mechanical effect</rdfs:label>
        <skos:definition>Effect of actions in the form of forces, stresses, or strains in structural members.</skos:definition>
    </owl:Class>
    


    <!-- http://www.w3id.org/eurocodes/ec1990#MediumVehicleTraffic -->


    <owl:Class rdf:about="http://www.w3id.org/eurocodes/ec1990#MediumVehicleTraffic">
        <rdfs:subClassOf rdf:resource="http://www.w3id.org/eurocodes/ec1990#EurocodeZone"/>
        <terms:source>EN 1991-1-1:2002 Table 6.7</terms:source>
        <rdfs:label xml:lang="en">Category G - medium vehicle traffic</rdfs:label>
        <skos:definition>Traffic and parking area for medium vehicles (&gt;30 kN, ≤ 160 kN gross vehicle weight, on 2 axles)</skos:definition>
        <skos:example>access routes, delivery zones, zones accessible to fire engines (≤ 160 kN gross vehicle weight)</skos:example>
    </owl:Class>
    


    <!-- http://www.w3id.org/eurocodes/ec1990#NominalValue -->


    <owl:Class rdf:about="http://www.w3id.org/eurocodes/ec1990#NominalValue">
        <rdfs:subClassOf rdf:resource="http://qudt.org/3.1.2/schema/qudt/QuantityValue"/>
        <rdfs:label xml:lang="en">Nominal value</rdfs:label>
        <skos:definition>A conventional or assigned value of a physical quantity used for reference in design.</skos:definition>
    </owl:Class>
    


    <!-- http://www.w3id.org/eurocodes/ec1990#NormalStress -->


    <owl:Class rdf:about="http://www.w3id.org/eurocodes/ec1990#NormalStress">
        <rdfs:subClassOf rdf:resource="http://www.w3id.org/eurocodes/ec1990#Stress"/>
        <rdfs:label xml:lang="en">Normal stress</rdfs:label>
        <skos:definition>Stress acting in the direction normal to a surface.</skos:definition>
    </owl:Class>
    


    <!-- http://www.w3id.org/eurocodes/ec1990#OfficeArea -->


    <owl:Class rdf:about="http://www.w3id.org/eurocodes/ec1990#OfficeArea">
        <rdfs:subClassOf rdf:resource="http://www.w3id.org/eurocodes/ec1990#EurocodeZone"/>
        <terms:source>EN 1991-1-1:2002 Table 6.1</terms:source>
        <rdfs:label xml:lang="en">Category B - office areas</rdfs:label>
        <skos:definition>Office area</skos:definition>
        <skos:example>General office spaces</skos:example>
    </owl:Class>
    


    <!-- http://www.w3id.org/eurocodes/ec1990#PermanentAction -->


    <owl:Class rdf:about="http://www.w3id.org/eurocodes/ec1990#PermanentAction">
        <rdfs:subClassOf rdf:resource="http://www.w3id.org/eurocodes/ec1990#Action"/>
        <owl:disjointWith rdf:resource="http://www.w3id.org/eurocodes/ec1990#VariableAction"/>
        <terms:source>EN 1990:2002, Section 1.5.3.3</terms:source>
        <rdfs:label xml:lang="en">Permanent action</rdfs:label>
        <skos:altLabel>G</skos:altLabel>
        <skos:definition>Action that is likely to act throughout a given reference period and for which the variation in magnitude with time is negligible, or for which the variation is always in the same direction (monotonic) until the action attains a certain limit value.</skos:definition>
        <skos:example>self-weight, fixed equipment</skos:example>
    </owl:Class>
    


    <!-- http://www.w3id.org/eurocodes/ec1990#PersistentDesignSituation -->


    <owl:Class rdf:about="http://www.w3id.org/eurocodes/ec1990#PersistentDesignSituation">
        <rdfs:subClassOf rdf:resource="http://www.w3id.org/eurocodes/ec1990#DesignSituation"/>
        <terms:source>EN 1990:2002, Section 1.5.2.4</terms:source>
        <rdfs:label xml:lang="en">Persistent design situation</rdfs:label>
        <skos:definition>Design situation that is relevant during a period of the same order as the design working life of the structure. Generally refers to conditions of normal use.</skos:definition>
    </owl:Class>
    


    <!-- http://www.w3id.org/eurocodes/ec1990#PhysicalActivitiesAreas -->


    <owl:Class rdf:about="http://www.w3id.org/eurocodes/ec1990#PhysicalActivitiesAreas">
        <rdfs:subClassOf rdf:resource="http://www.w3id.org/eurocodes/ec1990#CongregationArea"/>
        <terms:source>EN 1991-1-1:2002 Table 6.1</terms:source>
        <rdfs:label xml:lang="en">Category C4 - physical activities areas</rdfs:label>
        <skos:definition>Area with possible physical activities</skos:definition>
        <skos:example>dance halls, gymnastic rooms, stages</skos:example>
    </owl:Class>
    


    <!-- http://www.w3id.org/eurocodes/ec1990#PrincipalStress -->


    <owl:Class rdf:about="http://www.w3id.org/eurocodes/ec1990#PrincipalStress">
        <rdfs:subClassOf rdf:resource="http://www.w3id.org/eurocodes/ec1990#Stress"/>
        <rdfs:label xml:lang="en">Principal stress</rdfs:label>
        <skos:definition>Maximum or minimum normal stress at a point.</skos:definition>
    </owl:Class>
    


    <!-- http://www.w3id.org/eurocodes/ec1990#QuasiPermanentCombination -->


    <owl:Class rdf:about="http://www.w3id.org/eurocodes/ec1990#QuasiPermanentCombination">
        <rdfs:subClassOf rdf:resource="http://www.w3id.org/eurocodes/ec1990#SLSCombination"/>
        <terms:source>EN 1990:2002, Section 6.5.3(2)c</terms:source>
        <rdfs:label xml:lang="en">Quasi-permanent combination</rdfs:label>
        <skos:definition>Serviceability combination normally used for long-term effects and the appearance of the structure.</skos:definition>
        <skos:scopeNote>Used for long-term effects and appearance considerations</skos:scopeNote>
    </owl:Class>
    


    <!-- http://www.w3id.org/eurocodes/ec1990#QuasiStaticAction -->


    <owl:Class rdf:about="http://www.w3id.org/eurocodes/ec1990#QuasiStaticAction">
        <rdfs:subClassOf rdf:resource="http://www.w3id.org/eurocodes/ec1990#DynamicAction"/>
        <terms:source>EN 1990:2002, Section 1.5.3.13</terms:source>
        <rdfs:label xml:lang="en">Quasi-static action</rdfs:label>
        <skos:definition>Dynamic action represented by an equivalent static action in a static model.</skos:definition>
    </owl:Class>
    


    <!-- http://www.w3id.org/eurocodes/ec1990#Reaction -->


    <owl:Class rdf:about="http://www.w3id.org/eurocodes/ec1990#Reaction">
        <rdfs:subClassOf rdf:resource="http://www.w3id.org/eurocodes/ec1990#EffectOfAction"/>
        <terms:source>EN 1990:2002, Section 1.5.3.2</terms:source>
        <rdfs:label xml:lang="en">Reaction</rdfs:label>
        <skos:definition>Support reaction force or moment at structural supports.</skos:definition>
    </owl:Class>
    


    <!-- http://www.w3id.org/eurocodes/ec1990#RepresentativeAction -->


    <owl:Class rdf:about="http://www.w3id.org/eurocodes/ec1990#RepresentativeAction">
        <rdfs:subClassOf rdf:resource="http://www.w3id.org/eurocodes/ec1990#Action"/>
        <terms:source>EN 1990:2002, Section 1.5.3.20</terms:source>
        <rdfs:label xml:lang="en">Representative action</rdfs:label>
        <skos:definition>Value ofan action used for limit state verification. A representative value may be the characteristic value or an accompanying value.</skos:definition>
    </owl:Class>
    


    <!-- http://www.w3id.org/eurocodes/ec1990#RepresentativeValue -->


    <owl:Class rdf:about="http://www.w3id.org/eurocodes/ec1990#RepresentativeValue">
        <rdfs:subClassOf rdf:resource="http://qudt.org/3.1.2/schema/qudt/QuantityValue"/>
        <rdfs:label xml:lang="en">Representative value</rdfs:label>
        <skos:definition>A value that approximates a physical parameter in a way that reflects its expected role in structural analysis or verification.</skos:definition>
    </owl:Class>
    


    <!-- http://www.w3id.org/eurocodes/ec1990#Residential -->


    <owl:Class rdf:about="http://www.w3id.org/eurocodes/ec1990#Residential">
        <rdfs:subClassOf rdf:resource="http://www.w3id.org/eurocodes/ec1990#EurocodeZone"/>
        <terms:source>EN 1991-1-1:2002 Table 6.1</terms:source>
        <rdfs:label xml:lang="en">Category A - domestic and residential</rdfs:label>
        <skos:definition>Area for domestic and residential activities</skos:definition>
        <skos:example>rooms in residential buildings and houses, bedrooms and wards in hospitals, bedrooms in hotels and hostels, kitchens and toilets</skos:example>
    </owl:Class>
    


    <!-- http://www.w3id.org/eurocodes/ec1990#ResidentialBuilding -->


    <owl:Class rdf:about="http://www.w3id.org/eurocodes/ec1990#ResidentialBuilding">
        <rdfs:subClassOf rdf:resource="http://www.w3id.org/eurocodes/ec1990#Building"/>
        <terms:source>EN 1990:2002, Section 1.5.1.2</terms:source>
        <rdfs:label xml:lang="en">Residential building</rdfs:label>
        <skos:definition>Building intended primarily for the accommodation and permanent or temporary residence of individuals or households.</skos:definition>
        <skos:example>detached house, apartment building, high-rise residential tower</skos:example>
    </owl:Class>
    


    <!-- http://www.w3id.org/eurocodes/ec1990#Resistance -->


    <owl:Class rdf:about="http://www.w3id.org/eurocodes/ec1990#Resistance">
        <rdfs:subClassOf rdf:resource="http://www.w3id.org/eurocodes/ec1990#LimitStateValue"/>
        <terms:source>EN 1990:2002, Section 1.5.2.15</terms:source>
        <rdfs:label xml:lang="en">Resistance</rdfs:label>
        <skos:altLabel>R</skos:altLabel>
        <skos:definition>Capacity of a member or component, or a cross-section of a member or component of a structure, to withstand actions without mechanical failure.</skos:definition>
        <skos:example>bending resistance, buckling resistance, tension resistance</skos:example>
    </owl:Class>
    


    <!-- http://www.w3id.org/eurocodes/ec1990#Roof -->


    <owl:Class rdf:about="http://www.w3id.org/eurocodes/ec1990#Roof">
        <rdfs:subClassOf rdf:resource="http://www.w3id.org/eurocodes/ec1990#EurocodeZone"/>
        <terms:source>EN 1991-1-1:2002 Table 6.9</terms:source>
        <rdfs:label xml:lang="en">Category H - roofs</rdfs:label>
        <skos:definition>Roof not accessible except for normal maintenance and repair</skos:definition>
        <skos:example>roofs accessible only for maintenance</skos:example>
    </owl:Class>
    


    <!-- http://www.w3id.org/eurocodes/ec1990#Rotation -->


    <owl:Class rdf:about="http://www.w3id.org/eurocodes/ec1990#Rotation">
        <rdfs:subClassOf rdf:resource="http://www.w3id.org/eurocodes/ec1990#AngularDeformation"/>
        <terms:source>EN 1990:2002, Section 1.5.3.2</terms:source>
        <rdfs:label xml:lang="en">Rotation</rdfs:label>
        <skos:definition>Angular rotation of a structure or structural member.</skos:definition>
    </owl:Class>
    


    <!-- http://www.w3id.org/eurocodes/ec1990#SLSCombination -->


    <owl:Class rdf:about="http://www.w3id.org/eurocodes/ec1990#SLSCombination">
        <rdfs:subClassOf rdf:resource="http://www.w3id.org/eurocodes/ec1990#CombinationOfActions"/>
        <owl:disjointWith rdf:resource="http://www.w3id.org/eurocodes/ec1990#ULSCombination"/>
        <terms:source>EN 1990:2002, Section 6.5.3</terms:source>
        <rdfs:label xml:lang="en">Serviceability Limit State combination</rdfs:label>
        <skos:definition>Combinations of actions for verifying serviceability limit states.</skos:definition>
    </owl:Class>
    


    <!-- http://www.w3id.org/eurocodes/ec1990#SeismicAction -->


    <owl:Class rdf:about="http://www.w3id.org/eurocodes/ec1990#SeismicAction">
        <rdfs:subClassOf rdf:resource="http://www.w3id.org/eurocodes/ec1990#AccidentalAction"/>
        <terms:source>EN 1990:2002, Section 1.5.3.6</terms:source>
        <rdfs:label xml:lang="en">Seismic action</rdfs:label>
        <skos:altLabel>A_E</skos:altLabel>
        <skos:definition>Action that arises due to earthquake ground motions.</skos:definition>
    </owl:Class>
    


    <!-- http://www.w3id.org/eurocodes/ec1990#SeismicCombination -->


    <owl:Class rdf:about="http://www.w3id.org/eurocodes/ec1990#SeismicCombination">
        <rdfs:subClassOf rdf:resource="http://www.w3id.org/eurocodes/ec1990#ULSCombination"/>
        <terms:source>EN 1990:2002, Section 6.4.3.4</terms:source>
        <rdfs:label xml:lang="en">Seismic combination</rdfs:label>
        <skos:definition>Combination of actions for seismic design situations.</skos:definition>
        <skos:scopeNote>Used for seismic design situations in ULS verifications</skos:scopeNote>
    </owl:Class>
    


    <!-- http://www.w3id.org/eurocodes/ec1990#SeismicDesignSituation -->


    <owl:Class rdf:about="http://www.w3id.org/eurocodes/ec1990#SeismicDesignSituation">
        <rdfs:subClassOf rdf:resource="http://www.w3id.org/eurocodes/ec1990#DesignSituation"/>
        <terms:source>EN 1990:2002, Section 1.5.2.7</terms:source>
        <rdfs:label xml:lang="en">Seismic design situation</rdfs:label>
        <skos:definition>Design situation involving exceptional conditions of the structure when subjected to a seismic event.</skos:definition>
    </owl:Class>
    


    <!-- http://www.w3id.org/eurocodes/ec1990#SelfWeight -->


    <owl:Class rdf:about="http://www.w3id.org/eurocodes/ec1990#SelfWeight">
        <rdfs:subClassOf rdf:resource="http://www.w3id.org/eurocodes/ec1990#PermanentAction"/>
        <terms:source>EN 1991-1-1:2002</terms:source>
        <rdfs:label xml:lang="en">Self-weight</rdfs:label>
        <skos:definition>Weight of the structure itself, including all permanent construction elements, finishes, fixed equipment, and any other permanently attached components.</skos:definition>
    </owl:Class>
    


    <!-- http://www.w3id.org/eurocodes/ec1990#ServiceabilityLimitState -->


    <owl:Class rdf:about="http://www.w3id.org/eurocodes/ec1990#ServiceabilityLimitState">
        <rdfs:subClassOf rdf:resource="http://www.w3id.org/eurocodes/ec1990#LimitState"/>
        <owl:disjointWith rdf:resource="http://www.w3id.org/eurocodes/ec1990#UltimateLimitState"/>
        <terms:source>EN 1990:2002, Section 1.5.2.14</terms:source>
        <rdfs:label xml:lang="en">Serviceability Limit State</rdfs:label>
        <skos:altLabel>SLS</skos:altLabel>
        <skos:definition>State that correspond to conditions beyond which specified service requirements for a structure or structural member are no longer met.</skos:definition>
    </owl:Class>
    


    <!-- http://www.w3id.org/eurocodes/ec1990#ShearForce -->


    <owl:Class rdf:about="http://www.w3id.org/eurocodes/ec1990#ShearForce">
        <rdfs:subClassOf rdf:resource="http://www.w3id.org/eurocodes/ec1990#InternalForce"/>
        <terms:source>EN 1990:2002, Section 1.5.3.2</terms:source>
        <rdfs:label xml:lang="en">Shear force</rdfs:label>
        <skos:altLabel>V</skos:altLabel>
        <skos:definition>Internal force acting perpendicular to the axis of structural members.</skos:definition>
    </owl:Class>
    


    <!-- http://www.w3id.org/eurocodes/ec1990#ShearStress -->


    <owl:Class rdf:about="http://www.w3id.org/eurocodes/ec1990#ShearStress">
        <rdfs:subClassOf rdf:resource="http://www.w3id.org/eurocodes/ec1990#Stress"/>
        <rdfs:label xml:lang="en">Shear stress</rdfs:label>
        <skos:definition>Stress acting in the direction parallel (tangential) to a surface.</skos:definition>
    </owl:Class>
    


    <!-- http://www.w3id.org/eurocodes/ec1990#ShoppingAreas -->


    <owl:Class rdf:about="http://www.w3id.org/eurocodes/ec1990#ShoppingAreas">
        <rdfs:subClassOf rdf:resource="http://www.w3id.org/eurocodes/ec1990#EurocodeZone"/>
        <terms:source>EN 1991-1-1:2002 Table 6.1</terms:source>
        <rdfs:label xml:lang="en">Category D - shopping areas</rdfs:label>
        <skos:definition>Shopping area</skos:definition>
    </owl:Class>
    


    <!-- http://www.w3id.org/eurocodes/ec1990#ShrinkageEffect -->


    <owl:Class rdf:about="http://www.w3id.org/eurocodes/ec1990#ShrinkageEffect">
        <rdfs:subClassOf rdf:resource="http://www.w3id.org/eurocodes/ec1990#TimeDependentEffect"/>
        <rdfs:label xml:lang="en">Shrinkage effect</rdfs:label>
        <skos:definition>Deformation effect due to material shrinkage over time.</skos:definition>
    </owl:Class>
    


    <!-- http://www.w3id.org/eurocodes/ec1990#SnowLoad -->


    <owl:Class rdf:about="http://www.w3id.org/eurocodes/ec1990#SnowLoad">
        <rdfs:subClassOf rdf:resource="http://www.w3id.org/eurocodes/ec1990#VariableAction"/>
        <owl:disjointWith rdf:resource="http://www.w3id.org/eurocodes/ec1990#ThermalAction"/>
        <owl:disjointWith rdf:resource="http://www.w3id.org/eurocodes/ec1990#WindAction"/>
        <terms:source>EN 1991-1-3:2003</terms:source>
        <rdfs:label xml:lang="en">Snow load</rdfs:label>
        <skos:definition>Variable climatic action caused by the accumulation of snow on the surface of structures.</skos:definition>
    </owl:Class>
    


    <!-- http://www.w3id.org/eurocodes/ec1990#StaticAction -->


    <owl:Class rdf:about="http://www.w3id.org/eurocodes/ec1990#StaticAction">
        <rdfs:subClassOf rdf:resource="http://www.w3id.org/eurocodes/ec1990#Action"/>
        <terms:source>EN 1990:2002, Section 1.5.3.11</terms:source>
        <rdfs:label xml:lang="en">Static action</rdfs:label>
        <skos:definition>Action that does not cause significant acceleration of the structure or structural members.</skos:definition>
    </owl:Class>
    


    <!-- http://www.w3id.org/eurocodes/ec1990#StorageAreas -->


    <owl:Class rdf:about="http://www.w3id.org/eurocodes/ec1990#StorageAreas">
        <rdfs:subClassOf rdf:resource="http://www.w3id.org/eurocodes/ec1990#IndustrialandStorage"/>
        <terms:source>EN 1991-1-1:2002 Table 6.3</terms:source>
        <rdfs:label xml:lang="en">Category E1 - storage areas</rdfs:label>
        <skos:definition>Area susceptible to accumulation of goods, including access areas</skos:definition>
        <skos:example>areas for storage use including storage of books and other documents: archives, libraries, stockrooms</skos:example>
    </owl:Class>
    


    <!-- http://www.w3id.org/eurocodes/ec1990#Strain -->


    <owl:Class rdf:about="http://www.w3id.org/eurocodes/ec1990#Strain">
        <rdfs:subClassOf rdf:resource="http://www.w3id.org/eurocodes/ec1990#MechanicalEffect"/>
        <terms:source>EN 1990:2002, Section 1.5.3.2</terms:source>
        <rdfs:label xml:lang="en">Strain</rdfs:label>
        <skos:definition>Deformation per unit length in structural members.</skos:definition>
    </owl:Class>
    


    <!-- http://www.w3id.org/eurocodes/ec1990#Stress -->


    <owl:Class rdf:about="http://www.w3id.org/eurocodes/ec1990#Stress">
        <rdfs:subClassOf rdf:resource="http://www.w3id.org/eurocodes/ec1990#MechanicalEffect"/>
        <terms:source>EN 1990:2002, Section 1.5.3.2</terms:source>
        <rdfs:label xml:lang="en">Stress</rdfs:label>
        <skos:definition>Internal stress in structural members due to actions.</skos:definition>
    </owl:Class>
    


    <!-- http://www.w3id.org/eurocodes/ec1990#StructuralMember -->


    <owl:Class rdf:about="http://www.w3id.org/eurocodes/ec1990#StructuralMember">
        <rdfs:subClassOf rdf:resource="http://purl.obolibrary.org/obo/BFO_0000040"/>
        <rdfs:subClassOf rdf:resource="https://w3id.org/bot#Element"/>
        <terms:source>EN 1990:200, Section 1.5.1.7</terms:source>
        <rdfs:label xml:lang="en">Structural member</rdfs:label>
        <skos:definition>Physically distinguishable part of a structure, e.g. a column, a beam, a slab, a foundation pile.</skos:definition>
        <skos:example>column, beam, slab, foundation pile</skos:example>
    </owl:Class>
    


    <!-- http://www.w3id.org/eurocodes/ec1990#StructuralSystem -->


    <owl:Class rdf:about="http://www.w3id.org/eurocodes/ec1990#StructuralSystem">
        <rdfs:subClassOf rdf:resource="http://purl.obolibrary.org/obo/BFO_0000040"/>
        <terms:source>EN 1990:2002, Section 1.5.1.9</terms:source>
        <rdfs:label xml:lang="en">Structural system</rdfs:label>
        <skos:definition>Load-bearing members of a building or civil engineering works and the way in which these members function together.</skos:definition>
        <skos:example>Flat-slab system with drop panels, steel potal frame, cable-stayed bridge system, trussed roof system</skos:example>
    </owl:Class>
    


    <!-- http://www.w3id.org/eurocodes/ec1990#Structure -->


    <owl:Class rdf:about="http://www.w3id.org/eurocodes/ec1990#Structure">
        <rdfs:subClassOf rdf:resource="http://purl.obolibrary.org/obo/BFO_0000040"/>
        <terms:source>EN 1990:2002, Section 1.5.1.6</terms:source>
        <rdfs:label xml:lang="en">Structure</rdfs:label>
        <skos:definition>Organised combination of connected parts designed to carry loads and provide adequate rigidity.</skos:definition>
        <skos:example>Residential building, reatining wall, suspension bridge, underground tunnel</skos:example>
    </owl:Class>
    


    <!-- http://www.w3id.org/eurocodes/ec1990#ThermalAction -->


    <owl:Class rdf:about="http://www.w3id.org/eurocodes/ec1990#ThermalAction">
        <rdfs:subClassOf rdf:resource="http://www.w3id.org/eurocodes/ec1990#VariableAction"/>
        <owl:disjointWith rdf:resource="http://www.w3id.org/eurocodes/ec1990#WindAction"/>
        <terms:source>EN 1991-1-5:2003, Section 1.5.1</terms:source>
        <rdfs:label xml:lang="en">Thermal action</rdfs:label>
        <skos:definition>Actions that arises from the changes of temperature fields within a specified time interval.</skos:definition>
    </owl:Class>
    


    <!-- http://www.w3id.org/eurocodes/ec1990#Thickness -->


    <owl:Class rdf:about="http://www.w3id.org/eurocodes/ec1990#Thickness">
        <rdfs:subClassOf rdf:resource="http://www.w3id.org/eurocodes/ec1990#GeometricalProperty"/>
        <rdfs:label xml:lang="en">Thickness</rdfs:label>
        <skos:definition>Dimension of a structural element measured perpendicular to its plane or surface.</skos:definition>
    </owl:Class>
    


    <!-- http://www.w3id.org/eurocodes/ec1990#TimeDependentEffect -->


    <owl:Class rdf:about="http://www.w3id.org/eurocodes/ec1990#TimeDependentEffect">
        <rdfs:subClassOf rdf:resource="http://www.w3id.org/eurocodes/ec1990#EffectOfAction"/>
        <terms:source>EN 1990:2002, Section 3.1(5)</terms:source>
        <rdfs:label xml:lang="en">Time-dependent effect</rdfs:label>
        <skos:definition>Effect of actions that varies with time due to material behavior or other time-related factors.</skos:definition>
    </owl:Class>
    


    <!-- http://www.w3id.org/eurocodes/ec1990#TorsionalMoment -->


    <owl:Class rdf:about="http://www.w3id.org/eurocodes/ec1990#TorsionalMoment">
        <rdfs:subClassOf rdf:resource="http://www.w3id.org/eurocodes/ec1990#InternalForce"/>
        <terms:source>EN 1990:2002, Section 1.5.3.2</terms:source>
        <rdfs:label xml:lang="en">Torsional moment</rdfs:label>
        <skos:altLabel>T</skos:altLabel>
        <skos:definition>Internal moment causing twisting in structural members.</skos:definition>
    </owl:Class>
    


    <!-- http://www.w3id.org/eurocodes/ec1990#TransientDesignSituation -->


    <owl:Class rdf:about="http://www.w3id.org/eurocodes/ec1990#TransientDesignSituation">
        <rdfs:subClassOf rdf:resource="http://www.w3id.org/eurocodes/ec1990#DesignSituation"/>
        <terms:source>EN 1990:2002, Section 1.5.2.3</terms:source>
        <rdfs:label xml:lang="en">Transient design situation</rdfs:label>
        <skos:definition>Design situation that is relevant during a period much shorter than the design working life of the structure and which has a high probability of occurrence, e.g. during construction or repair.</skos:definition>
        <skos:example>construction phase, repair operations</skos:example>
    </owl:Class>
    


    <!-- http://www.w3id.org/eurocodes/ec1990#Twist -->


    <owl:Class rdf:about="http://www.w3id.org/eurocodes/ec1990#Twist">
        <rdfs:subClassOf rdf:resource="http://www.w3id.org/eurocodes/ec1990#AngularDeformation"/>
        <rdfs:label xml:lang="en">Twist</rdfs:label>
        <skos:definition>Angular deformation about the longitudinal axis.</skos:definition>
    </owl:Class>
    


    <!-- http://www.w3id.org/eurocodes/ec1990#ULSCombination -->


    <owl:Class rdf:about="http://www.w3id.org/eurocodes/ec1990#ULSCombination">
        <rdfs:subClassOf rdf:resource="http://www.w3id.org/eurocodes/ec1990#CombinationOfActions"/>
        <terms:source>EN 1990:2002, Section 6.4.3</terms:source>
        <rdfs:label xml:lang="en">Ultimate Limit State combination</rdfs:label>
        <skos:definition>Combination of actions for verifying ultimate limit states.</skos:definition>
    </owl:Class>
    


    <!-- http://www.w3id.org/eurocodes/ec1990#UltimateLimitState -->


    <owl:Class rdf:about="http://www.w3id.org/eurocodes/ec1990#UltimateLimitState">
        <rdfs:subClassOf rdf:resource="http://www.w3id.org/eurocodes/ec1990#LimitState"/>
        <terms:source>EN 1990:2002, Section 1.5.2.13</terms:source>
        <rdfs:label xml:lang="en">Ultimate Limit State</rdfs:label>
        <skos:altLabel>ULS</skos:altLabel>
        <skos:definition>State associated with collapse or with other similar forms of structural failure. They generally correspond to the maximum load-carrying resistance of a structure or structural member.</skos:definition>
    </owl:Class>
    


    <!-- http://www.w3id.org/eurocodes/ec1990#UnfavourableAction -->


    <owl:Class rdf:about="http://www.w3id.org/eurocodes/ec1990#UnfavourableAction">
        <rdfs:subClassOf rdf:resource="http://www.w3id.org/eurocodes/ec1990#Action"/>
        <terms:source>EN 1990:2002, Section 6.3.2(3)P</terms:source>
        <rdfs:label xml:lang="en">UnfavourableAction action</rdfs:label>
        <skos:definition>An action that increases the effect of other actions on a structure, or otherwise reduces structural safety.</skos:definition>
    </owl:Class>
    


    <!-- http://www.w3id.org/eurocodes/ec1990#UpperBoundValue -->


    <owl:Class rdf:about="http://www.w3id.org/eurocodes/ec1990#UpperBoundValue">
        <rdfs:subClassOf rdf:resource="http://qudt.org/3.1.2/schema/qudt/QuantityValue"/>
        <rdfs:label xml:lang="en">Upper bound value</rdfs:label>
        <skos:definition>A conservative or code-specified maximum value of a physical quantity, used to limit overestimation of capacity or underestimation of actions.</skos:definition>
    </owl:Class>
    


    <!-- http://www.w3id.org/eurocodes/ec1990#VariableAction -->


    <owl:Class rdf:about="http://www.w3id.org/eurocodes/ec1990#VariableAction">
        <rdfs:subClassOf rdf:resource="http://www.w3id.org/eurocodes/ec1990#Action"/>
        <terms:source>EN 1990:2002, Section 1.5.3.4</terms:source>
        <rdfs:label xml:lang="en">Variable action</rdfs:label>
        <skos:altLabel>Q</skos:altLabel>
        <skos:definition>Action for which the variation in magnitude with time is neither negligible nor monotonic.</skos:definition>
        <skos:example>imposed loads, wind, snow, thermal actions</skos:example>
    </owl:Class>
    


    <!-- http://www.w3id.org/eurocodes/ec1990#VibrationResponse -->


    <owl:Class rdf:about="http://www.w3id.org/eurocodes/ec1990#VibrationResponse">
        <rdfs:subClassOf rdf:resource="http://www.w3id.org/eurocodes/ec1990#DynamicEffect"/>
        <rdfs:label xml:lang="en">Vibration response</rdfs:label>
        <skos:definition>Dynamic response of structures to oscillatory actions, important for serviceability considerations.</skos:definition>
    </owl:Class>
    


    <!-- http://www.w3id.org/eurocodes/ec1990#VolumetricDeformation -->


    <owl:Class rdf:about="http://www.w3id.org/eurocodes/ec1990#VolumetricDeformation">
        <rdfs:subClassOf rdf:resource="http://www.w3id.org/eurocodes/ec1990#Deformation"/>
        <rdfs:label xml:lang="en">Volumetric Deformation</rdfs:label>
        <skos:definition>Deformation involving change in volume of structural elements.</skos:definition>
    </owl:Class>
    


    <!-- http://www.w3id.org/eurocodes/ec1990#WindAction -->


    <owl:Class rdf:about="http://www.w3id.org/eurocodes/ec1990#WindAction">
        <rdfs:subClassOf rdf:resource="http://www.w3id.org/eurocodes/ec1990#VariableAction"/>
        <terms:source>EN 1991-1-4:2005</terms:source>
        <rdfs:label xml:lang="en">Wind action</rdfs:label>
        <skos:definition>Variable climatic action resulting from the movement of air relative to the surface of the Earth. These action acts as external pressure or suction on surfaces and can also induce internal pressure.</skos:definition>
    </owl:Class>
    


    <!-- 
    ///////////////////////////////////////////////////////////////////////////////////////
    //
    // Individuals
    //
    ///////////////////////////////////////////////////////////////////////////////////////
     -->


    


    <!-- http://www.w3id.org/eurocodes/ec1990#AgriculturalStructure -->


    <owl:NamedIndividual rdf:about="http://www.w3id.org/eurocodes/ec1990#AgriculturalStructure">
        <rdf:type rdf:resource="http://www.w3id.org/eurocodes/ec1990#Structure"/>
        <terms:source>EN 1990:2002, Table 2.1</terms:source>
        <rdfs:label xml:lang="en">Agricultural structure</rdfs:label>
        <skos:definition>A building or construction primarily designed and used for farming-related activities.</skos:definition>
        <skos:example>barn, greenhouse, animal shelter</skos:example>
    </owl:NamedIndividual>
    


    <!-- http://www.w3id.org/eurocodes/ec1990#BridgeStructure -->


    <owl:NamedIndividual rdf:about="http://www.w3id.org/eurocodes/ec1990#BridgeStructure">
        <rdf:type rdf:resource="http://www.w3id.org/eurocodes/ec1990#Structure"/>
        <terms:source>EN 1990:2002, Table 2.1</terms:source>
        <rdfs:label xml:lang="en">Bridge structure</rdfs:label>
        <skos:definition>Engineered construction designed to span physical obstacles such as rivers, valleys, roads, or railways, providing a safe passage for vehicles, pedestrians, or utilities.</skos:definition>
        <skos:example>beam bridge, arch bridge, suspension bridge</skos:example>
    </owl:NamedIndividual>
    


    <!-- http://www.w3id.org/eurocodes/ec1990#Building -->


    <owl:NamedIndividual rdf:about="http://www.w3id.org/eurocodes/ec1990#Building">
        <owl:sameAs rdf:resource="https://w3id.org/bot#Building"/>
    </owl:NamedIndividual>
    


    <!-- https://w3id.org/bot#Building -->


    <owl:NamedIndividual rdf:about="https://w3id.org/bot#Building"/>
    


    <!-- http://www.w3id.org/eurocodes/ec1990#BuildingStructure -->


    <owl:NamedIndividual rdf:about="http://www.w3id.org/eurocodes/ec1990#BuildingStructure">
        <rdf:type rdf:resource="http://www.w3id.org/eurocodes/ec1990#Structure"/>
        <terms:source>EN 1990:2002, Table 2.1</terms:source>
        <rdfs:label xml:lang="en">Building structure</rdfs:label>
        <skos:definition>Load-bearing framework or system designed to support and transfer all applied loads safely to the foundation and ultimately to the ground.</skos:definition>
        <skos:example>masonry building, steel frame building, timber-framed house</skos:example>
    </owl:NamedIndividual>
    


    <!-- http://www.w3id.org/eurocodes/ec1990#CivilEngineeringStructure -->


    <owl:NamedIndividual rdf:about="http://www.w3id.org/eurocodes/ec1990#CivilEngineeringStructure">
        <rdf:type rdf:resource="http://www.w3id.org/eurocodes/ec1990#Structure"/>
        <terms:source>EN 1990:2002, Table 2.1</terms:source>
        <rdfs:label xml:lang="en">Civil engineering structure</rdfs:label>
        <skos:definition>Constructed system composed of interconnected physical elements designed, analyzed, and built to withstand environmental and operational loads, enabling the provision of essential services such as transport, shelter, water management, or energy distribution.</skos:definition>
        <skos:example>dam, tunnel, airport, retaining wall, power station, road</skos:example>
    </owl:NamedIndividual>
    


    <!-- http://www.w3id.org/eurocodes/ec1990#EQU -->


    <owl:NamedIndividual rdf:about="http://www.w3id.org/eurocodes/ec1990#EQU">
        <rdf:type rdf:resource="http://www.w3id.org/eurocodes/ec1990#UltimateLimitState"/>
        <terms:source>EN 1990:2002, Section 6.4.1(1)P a)</terms:source>
        <rdfs:label xml:lang="en">Static equilibrium</rdfs:label>
        <skos:definition>Loss of static equilibrium of the structure or any part of it considered as a rigid body.</skos:definition>
    </owl:NamedIndividual>
    


    <!-- http://www.w3id.org/eurocodes/ec1990#Execution -->


    <owl:NamedIndividual rdf:about="http://www.w3id.org/eurocodes/ec1990#Execution">
        <rdf:type rdf:resource="http://www.w3id.org/eurocodes/ec1990#TransientDesignSituation"/>
        <terms:source>EN 1990:2002, Section 3.2(2)P</terms:source>
        <rdfs:label xml:lang="en">Execution</rdfs:label>
        <skos:definition>Transient design situation during execution of a construction work.</skos:definition>
    </owl:NamedIndividual>
    


    <!-- http://www.w3id.org/eurocodes/ec1990#ExplosionDesignSituation -->


    <owl:NamedIndividual rdf:about="http://www.w3id.org/eurocodes/ec1990#ExplosionDesignSituation">
        <rdf:type rdf:resource="http://www.w3id.org/eurocodes/ec1990#AccidentalDesignSituation"/>
        <terms:source>EN 1990:2002, Section 1.5.2.5</terms:source>
        <rdfs:label xml:lang="en">Explosion design situation</rdfs:label>
        <skos:definition>Accidental design situation involving explosion conditions.</skos:definition>
    </owl:NamedIndividual>
    


    <!-- http://www.w3id.org/eurocodes/ec1990#FAT -->


    <owl:NamedIndividual rdf:about="http://www.w3id.org/eurocodes/ec1990#FAT">
        <rdf:type rdf:resource="http://www.w3id.org/eurocodes/ec1990#UltimateLimitState"/>
        <terms:source>EN 1990:2002, Section 6.4.1(1)P d)</terms:source>
        <rdfs:label xml:lang="en">Fatigue failure</rdfs:label>
        <skos:definition>Fatigue failure of the structure or structural members.</skos:definition>
    </owl:NamedIndividual>
    


    <!-- http://www.w3id.org/eurocodes/ec1990#FireDesignSituation -->


    <owl:NamedIndividual rdf:about="http://www.w3id.org/eurocodes/ec1990#FireDesignSituation">
        <rdf:type rdf:resource="http://www.w3id.org/eurocodes/ec1990#AccidentalDesignSituation"/>
        <terms:source>EN 1990:2002, Section 1.5.2.5 &amp; 6</terms:source>
        <rdfs:label xml:lang="en">Fire design situation</rdfs:label>
        <skos:definition>Accidental design situation involving fire conditions requiring specific design considerations.</skos:definition>
    </owl:NamedIndividual>
    


    <!-- http://www.w3id.org/eurocodes/ec1990#GEO -->


    <owl:NamedIndividual rdf:about="http://www.w3id.org/eurocodes/ec1990#GEO">
        <rdf:type rdf:resource="http://www.w3id.org/eurocodes/ec1990#UltimateLimitState"/>
        <terms:source>EN 1990:2002, Section 6.4.1(1)P c)</terms:source>
        <rdfs:label xml:lang="en">Geotechnical failure</rdfs:label>
        <skos:definition>Failure or excessive deformation of the ground where the strengths of soil or rock are significant in providing resistance.</skos:definition>
    </owl:NamedIndividual>
    


    <!-- http://www.w3id.org/eurocodes/ec1990#HYD -->


    <owl:NamedIndividual rdf:about="http://www.w3id.org/eurocodes/ec1990#HYD">
        <rdf:type rdf:resource="http://www.w3id.org/eurocodes/ec1990#UltimateLimitState"/>
        <terms:source>EN 1990:2002/A1:2005, Section 6.4.1(1)P f)</terms:source>
        <rdfs:label xml:lang="en">Hydraulic failure</rdfs:label>
        <skos:definition>Hydraulic heave, internal erosion and piping in the ground caused by hydraulic gradients.</skos:definition>
    </owl:NamedIndividual>
    


    <!-- http://www.w3id.org/eurocodes/ec1990#ISLS -->


    <owl:NamedIndividual rdf:about="http://www.w3id.org/eurocodes/ec1990#ISLS">
        <rdf:type rdf:resource="http://www.w3id.org/eurocodes/ec1990#ServiceabilityLimitState"/>
        <terms:source>EN 1990:2002, Section 1.5.2.14.1</terms:source>
        <rdfs:label xml:lang="en">Irreversible Serviceability Limit State</rdfs:label>
        <skos:definition>Serviceability limit state where some consequences of actions exceeding the specified service requirements will remain when the actions are removed.</skos:definition>
    </owl:NamedIndividual>
    


    <!-- http://www.w3id.org/eurocodes/ec1990#ImpactDesignSituation -->


    <owl:NamedIndividual rdf:about="http://www.w3id.org/eurocodes/ec1990#ImpactDesignSituation">
        <rdf:type rdf:resource="http://www.w3id.org/eurocodes/ec1990#AccidentalDesignSituation"/>
        <terms:source>EN 1990:2002, Section 1.5.2.5</terms:source>
        <rdfs:label xml:lang="en">Impact design situation</rdfs:label>
        <skos:definition>Accidental design situation involving impact conditions.</skos:definition>
    </owl:NamedIndividual>
    


    <!-- http://www.w3id.org/eurocodes/ec1990#LocalizedFailureDesignSituation -->


    <owl:NamedIndividual rdf:about="http://www.w3id.org/eurocodes/ec1990#LocalizedFailureDesignSituation">
        <rdf:type rdf:resource="http://www.w3id.org/eurocodes/ec1990#AccidentalDesignSituation"/>
        <terms:source>EN 1990:2002, Section 1.5.2.5</terms:source>
        <rdfs:label xml:lang="en">Localized failure design situation</rdfs:label>
        <skos:definition>Accidental design situation involving local failure conditions.</skos:definition>
    </owl:NamedIndividual>
    


    <!-- http://www.w3id.org/eurocodes/ec1990#MonumentalBuldingStructure -->


    <owl:NamedIndividual rdf:about="http://www.w3id.org/eurocodes/ec1990#MonumentalBuldingStructure">
        <rdf:type rdf:resource="http://www.w3id.org/eurocodes/ec1990#Structure"/>
        <terms:source>EN 1990:2002, Table 2.1</terms:source>
        <rdfs:label xml:lang="en">Monumental building structure</rdfs:label>
        <skos:definition>Large-scale, architecturally significant structure designed to serve as a landmark, memorial, or symbol of cultural, historical, or civic importance.</skos:definition>
        <skos:example>national parliment building, museum of significant importance, major cathedral</skos:example>
    </owl:NamedIndividual>
    


    <!-- http://www.w3id.org/eurocodes/ec1990#RSLS -->


    <owl:NamedIndividual rdf:about="http://www.w3id.org/eurocodes/ec1990#RSLS">
        <rdf:type rdf:resource="http://www.w3id.org/eurocodes/ec1990#ServiceabilityLimitState"/>
        <terms:source>EN 1990:2002, Section 1.5.2.14.2</terms:source>
        <rdfs:label xml:lang="en">Reversible Serviceability Limit State</rdfs:label>
        <skos:definition>Serviceability limit state where no consequences of actions exceeding the specified service requirements will remain when the actions are removed.</skos:definition>
    </owl:NamedIndividual>
    


    <!-- http://www.w3id.org/eurocodes/ec1990#Repair -->


    <owl:NamedIndividual rdf:about="http://www.w3id.org/eurocodes/ec1990#Repair">
        <rdf:type rdf:resource="http://www.w3id.org/eurocodes/ec1990#TransientDesignSituation"/>
        <terms:source>EN 1990:2002, Section 3.2(2)P</terms:source>
        <rdfs:label xml:lang="en">Repair</rdfs:label>
        <skos:definition>Transient design situation during repair of a construction work.</skos:definition>
    </owl:NamedIndividual>
    


    <!-- http://www.w3id.org/eurocodes/ec1990#ReplacableStructuralElements -->


    <owl:NamedIndividual rdf:about="http://www.w3id.org/eurocodes/ec1990#ReplacableStructuralElements">
        <rdf:type rdf:resource="http://www.w3id.org/eurocodes/ec1990#Structure"/>
        <terms:source>EN 1990:2002, Table 2.1</terms:source>
        <rdfs:label xml:lang="en">Structure with replaceable elements</rdfs:label>
        <skos:definition>Structure designed such that certain primary or secondary structural components can be removed, replaced, or upgraded during its service life without compromising the overall stability, integrity, or usability of the structure.</skos:definition>
        <skos:example>modular steel bridge with replaceable girders, industrial building with precast concrete roof panels</skos:example>
    </owl:NamedIndividual>
    


    <!-- http://www.w3id.org/eurocodes/ec1990#STR -->


    <owl:NamedIndividual rdf:about="http://www.w3id.org/eurocodes/ec1990#STR">
        <rdf:type rdf:resource="http://www.w3id.org/eurocodes/ec1990#UltimateLimitState"/>
        <terms:source>EN 1990:2002, Section 6.4.1(1)P b)</terms:source>
        <rdfs:label xml:lang="en">Structural resistance</rdfs:label>
        <skos:definition>Internal failure or excessive deformation of the structure or structural members where the strength of construction materials governs.</skos:definition>
    </owl:NamedIndividual>
    


    <!-- http://www.w3id.org/eurocodes/ec1990#TemporaryStructure -->


    <owl:NamedIndividual rdf:about="http://www.w3id.org/eurocodes/ec1990#TemporaryStructure">
        <rdf:type rdf:resource="http://www.w3id.org/eurocodes/ec1990#Structure"/>
        <terms:source>EN 1990:2002, Table 2.1</terms:source>
        <rdfs:label xml:lang="en">Temporary structure</rdfs:label>
        <skos:definition>Structre that is intended to be used for a limited period of time, typically to support, protect, or provide access during the execution of permanent works, or to serve a short-term purpose.</skos:definition>
        <skos:example>formwork system, steel scaffolding, temoprary bridge</skos:example>
    </owl:NamedIndividual>
    


    <!-- http://www.w3id.org/eurocodes/ec1990#UPL -->


    <owl:NamedIndividual rdf:about="http://www.w3id.org/eurocodes/ec1990#UPL">
        <rdf:type rdf:resource="http://www.w3id.org/eurocodes/ec1990#UltimateLimitState"/>
        <terms:source>EN 1990:2002/A1:2005, Section 6.4.1(1)P e)</terms:source>
        <rdfs:label xml:lang="en">Uplift failure</rdfs:label>
        <skos:definition>Loss of equilibrium of the structure or the ground due to uplift by water pressure (buoyancy) or other vertical actions.</skos:definition>
    </owl:NamedIndividual>
    


    <!-- https://w3id.org/bot#Building -->


    <owl:NamedIndividual rdf:about="https://w3id.org/bot#Building"/>
    


    <!-- 
    ///////////////////////////////////////////////////////////////////////////////////////
    //
    // Annotations
    //
    ///////////////////////////////////////////////////////////////////////////////////////
     -->


    <rdf:Description rdf:about="http://www.w3id.org/eurocodes/ec1990#Building">
        <terms:source>EN 1990:2002, Section 1.5.1.2</terms:source>
        <rdfs:label xml:lang="en">Building</rdfs:label>
        <skos:definition>Type of construction work for building purposes such as dwelling houses, office buildings, etc.</skos:definition>
        <skos:example>dwelling house, office building, industrial building</skos:example>
    </rdf:Description>
</rdf:RDF>



<!-- Generated by the OWL API (version 5.1.18) https://github.com/owlcs/owlapi/ -->


